@prefix : <http://www.wings-workflows.org/ontology/workflow.owl#> .
@prefix owl: <http://www.w3.org/2002/07/owl#> .
@prefix rdf: <http://www.w3.org/1999/02/22-rdf-syntax-ns#> .
@prefix xml: <http://www.w3.org/XML/1998/namespace> .
@prefix xsd: <http://www.w3.org/2001/XMLSchema#> .
@prefix rdfs: <http://www.w3.org/2000/01/rdf-schema#> .
@base <http://www.wings-workflows.org/ontology/workflow.owl> .

<http://www.wings-workflows.org/ontology/workflow.owl> rdf:type owl:Ontology .

#################################################################
#    Annotation properties
#################################################################

###  http://www.w3.org/2000/01/rdf-schema#comment
rdfs:comment rdf:type owl:AnnotationProperty .


###  http://www.w3.org/2004/02/skos/core#example
<http://www.w3.org/2004/02/skos/core#example> rdf:type owl:AnnotationProperty .


#################################################################
#    Object Properties
#################################################################

###  http://www.wings-workflows.org/ontology/workflow.owl#breakPoint
:breakPoint rdf:type owl:ObjectProperty ;
            rdfs:domain :Variable ;
            rdfs:range xsd:true .


###  http://www.wings-workflows.org/ontology/workflow.owl#canRunOn
:canRunOn rdf:type owl:ObjectProperty ;
          rdfs:domain :Node ;
          rdfs:range <http://www.wings-workflows.org/ontology/resource.owl#Machine> ;
          rdfs:label "canRunOn"^^xsd:string ;
          <http://www.w3.org/2004/02/skos/core#example> """
      @prefix workflow: <http://www.wings-workflows.org/ontology/workflow.owl#> .

      <http://ontosoft.isi.edu:8080/wings-portal/export/users/tirth/TestingDomain/executions/abstractTest1-83-7336709c-6108-4fc8-9ecd-810f27c8d870.owl#countingWordsNode>
            a workflow:Node ;
        rdfs:comment 
          \"center:x=262.99648571014404,y=280.32958602905273\"^^xsd:string ;
        workflow:hasComponent 
          <http://ontosoft.isi.edu:8080/wings-portal/export/users/tirth/TestingDomain/executions/abstractTest1-83-7336709c-6108-4fc8-9ecd-810f27c8d870.owl#countingWords> ;
        workflow:hasInputPort 
          <http://ontosoft.isi.edu:8080/wings-portal/export/users/tirth/TestingDomain/executions/abstractTest1-83-7336709c-6108-4fc8-9ecd-810f27c8d870.owl#countingWords_node_InputTextFile_0001>, <http://ontosoft.isi.edu:8080/wings-portal/export/users/tirth/TestingDomain/executions/abstractTest1-83-7336709c-6108-4fc8-9ecd-810f27c8d870.owl#countingWords_node_WordInput_0001> ;
        workflow:hasOutputPort 
          <http://ontosoft.isi.edu:8080/wings-portal/export/users/tirth/TestingDomain/executions/abstractTest1-83-7336709c-6108-4fc8-9ecd-810f27c8d870.owl#countingWords_node_OutputTextFile_1> ;
        workflow:canRunOn 
          <http://www.wings-workflows.org/ontology/resource.owl#Localhost> ;
        workflow:derivedFrom 
          <http://ontosoft.isi.edu:8080/wings-portal/export/users/tirth/TestingDomain/workflows/abstractTest1.owl#countingWords_node> .
    """^^xsd:string .


###  http://www.wings-workflows.org/ontology/workflow.owl#createSetsOn
:createSetsOn rdf:type owl:ObjectProperty ;
              rdfs:domain :SetCreationRule ;
              rdfs:range [ rdf:type owl:Class ;
                           owl:unionOf ( :ComponentVariable
                                         :SetCreationExpression
                                       )
                         ] ;
              rdfs:comment "The WINGS createSetsOn is a WINGS workflow object property that represents a connection between a WingsWorkflow SetCreationRule and a Component Variable i.e. a WingsWorkflowNode createSetsOn a WingsWorkflowComponentVariable."^^xsd:string ;
              rdfs:label "createSetsOn"^^xsd:string ;
              <http://www.w3.org/2004/02/skos/core#example> """
      @prefix workflow: <http://www.wings-workflows.org/ontology/workflow.owl#> .

      <http://ontosoft.isi.edu:8080/wings-portal/export/users/
      tirth/TestingDomain/workflows/r1.owl#xmltotext_node_crule>
            a workflow:ComponentSetRule ;
        workflow:createSetsOn 
          <http://ontosoft.isi.edu:8080/wings-portal/
          export/users/tirth/TestingDomain/workflows/r1.owl#xmltotext_node_comp> ;
        workflow:createWorkflowSets 
          true .

        """^^xsd:string .


###  http://www.wings-workflows.org/ontology/workflow.owl#derivedFrom
:derivedFrom rdf:type owl:ObjectProperty ;
             rdfs:label "derivedFrom"^^xsd:string ;
             <http://www.w3.org/2004/02/skos/core#example> """
    @prefix workflow: <http://www.wings-workflows.org/ontology/workflow.owl#> .
    
    <http://ontosoft.isi.edu:8080/wings-portal/export/users/tirth/TestingDomain/executions/abstractTest1-83-7336709c-6108-4fc8-9ecd-810f27c8d870.owl#htmltotextNode>
          a workflow:Node ;
      rdfs:comment 
        \"center:x=160.701757144928,y=113.66397857666016\"^^xsd:string ;
      workflow:hasComponent 
        <http://ontosoft.isi.edu:8080/wings-portal/export/users/tirth/TestingDomain/executions/abstractTest1-83-7336709c-6108-4fc8-9ecd-810f27c8d870.owl#htmltotext> ;
      workflow:hasInputPort 
        <http://ontosoft.isi.edu:8080/wings-portal/export/users/tirth/TestingDomain/executions/abstractTest1-83-7336709c-6108-4fc8-9ecd-810f27c8d870.owl#ConvertToText_node_InputFormattedFile_0000> ;
      workflow:hasOutputPort 
        <http://ontosoft.isi.edu:8080/wings-portal/export/users/tirth/TestingDomain/executions/abstractTest1-83-7336709c-6108-4fc8-9ecd-810f27c8d870.owl#ConvertToText_node_OutputTextFile_0> ;
      workflow:canRunOn 
        <http://www.wings-workflows.org/ontology/resource.owl#Localhost> ;
      workflow:derivedFrom 
        <http://ontosoft.isi.edu:8080/wings-portal/export/users/tirth/TestingDomain/workflows/abstractTest1.owl#ConvertToText_node> .
  """^^xsd:string .


###  http://www.wings-workflows.org/ontology/workflow.owl#hasComponent
:hasComponent rdf:type owl:ObjectProperty ,
                       owl:FunctionalProperty ;
              rdfs:domain :Node ;
              rdfs:range :ComponentVariable ;
              rdfs:comment "The WINGS hasComponent is a WINGS workflow object property that represents a connection between a WingsWorkflow Node and a Component Variable i.e. a WingsWorkflowNode hasComponent a WingsWorkflowComponentVariable."^^xsd:string ;
              rdfs:label "hasComponent"^^xsd:string ;
              <http://www.w3.org/2004/02/skos/core#example> """

        @prefix workflow: <http://www.wings-workflows.org/ontology/workflow.owl#> .
        @prefix rdfs: <http://www.w3.org/2000/01/rdf-schema#> .

        <http://ontosoft.isi.edu:8080/wings-portal/export/users/tirth/TestingDomain/workflows/r1.owl#xmltotext_node>
              a workflow:Node ;
          rdfs:comment 
            \"center:x=220,y=130\"^^xsd:string ;
          workflow:hasComponent 
            <http://ontosoft.isi.edu:8080/wings-portal/export/users/tirth/TestingDomain/workflows/
            r1.owl#xmltotext_node_comp> ;
          workflow:hasComponentSetCreationRule 
            <http://ontosoft.isi.edu:8080/wings-portal/export/users/tirth/TestingDomain/workflows/r1.owl#xmltotext_node_crule> ;
          workflow:hasInputPort 
            <http://ontosoft.isi.edu:8080/wings-portal/export/users/tirth/TestingDomain/workflows/r1.owl#xmltotext_node_InputFormattedFile> ;
          workflow:hasOutputPort 
            <http://ontosoft.isi.edu:8080/wings-portal/export/users/tirth/TestingDomain/workflows/r1.owl#xmltotext_node_OutputTextFile> ;
          workflow:hasPortSetCreationRule 
            <http://ontosoft.isi.edu:8080/wings-portal/export/users/tirth/TestingDomain/workflows/r1.owl#xmltotext_node_prule> . 
       """^^xsd:string .


###  http://www.wings-workflows.org/ontology/workflow.owl#hasComponentBinding
:hasComponentBinding rdf:type owl:ObjectProperty ;
                     rdfs:domain :ComponentVariable ;
                     rdfs:comment "The WINGS hasComponentBinding is a WINGS workflow object property that represents a connection between a WingsWorkflowComponentVariable and a ComponentBinding i.e. a WingsWorkflowComponentVariable hasComponentBinding WingsWorkflowComponentBinding."^^xsd:string ;
                     rdfs:label "hasComponentBinding"^^xsd:string ;
                     <http://www.w3.org/2004/02/skos/core#example> """
        @prefix workflow: <http://www.wings-workflows.org/ontology/workflow.owl#> .

        <http://ontosoft.isi.edu:8080/wings-portal/export/users/tirth/TestingDomain/workflows/s6.owl#third_node_comp>
            workflow:hasComponentBinding 
              <http://ontosoft.isi.edu:8080/wings-portal/export/users/tirth/TestingDomain/components/
              library.owl#third> ;
            workflow:isConcrete 
              true .
    """^^xsd:string .


###  http://www.wings-workflows.org/ontology/workflow.owl#hasComponentSetCreationRule
:hasComponentSetCreationRule rdf:type owl:ObjectProperty ;
                             rdfs:domain :Node ;
                             rdfs:range :SetCreationRule ;
                             rdfs:comment "The WINGS hasComponentSetCreationRule is a WINGS workflow object property that represents a connection between a WingsWorkflowNode and a SetCreationRule i.e. a WingsWorkflowNode hasComponentSetCreationRule SetCreationRule."^^xsd:string ;
                             rdfs:label "hasComponentSetCreationRule"^^xsd:string ;
                             <http://www.w3.org/2004/02/skos/core#example> """
          @prefix workflow: <http://www.wings-workflows.org/ontology/workflow.owl#> .

          <http://ontosoft.isi.edu:8080/wings-portal/export/users/tirth/TestingDomain/workflows/s6.owl#third_node>
                a workflow:Node ;
            rdfs:comment 
              \"center:x=314,y=148\"^^xsd:string ;
            workflow:hasComponent 
              <http://ontosoft.isi.edu:8080/wings-portal/export/users/tirth/TestingDomain/workflows/s6.owl#third_node_comp> ;
            workflow:hasComponentSetCreationRule 
              <http://ontosoft.isi.edu:8080/wings-portal/export/users/tirth/TestingDomain/workflows/s6.owl#third_node_crule> ;
            workflow:hasInputPort 
              <http://ontosoft.isi.edu:8080/wings-portal/export/users/tirth/TestingDomain/workflows/
              s6.owl#third_node_SecondInputFile>, <http://ontosoft.isi.edu:8080/wings-portal/export/users/tirth/
              TestingDomain/workflows/s6.owl#third_node_InputFile>, <http://ontosoft.isi.edu:8080/wings-portal/export/users
              /tirth/TestingDomain/workflows/s6.owl#third_node_InputWord> ;
            workflow:hasOutputPort 
              <http://ontosoft.isi.edu:8080/wings-portal/export/users/tirth/TestingDomain/workflows/
              s6.owl#third_node_OutputFile> ;
            workflow:hasPortSetCreationRule 
              <http://ontosoft.isi.edu:8080/wings-portal/export/users/tirth/TestingDomain/workflows/s6.owl#third_node_prule> .
      """^^xsd:string .


###  http://www.wings-workflows.org/ontology/workflow.owl#hasDataBinding
:hasDataBinding rdf:type owl:ObjectProperty ;
                rdfs:domain :DataVariable ;
                rdfs:label "hasDataBinding"^^xsd:string ;
                <http://www.w3.org/2004/02/skos/core#example> """
      @prefix owl: <http://www.w3.org/2002/07/owl#> .
      @prefix workflow: <http://www.wings-workflows.org/ontology/workflow.owl#> .
      @prefix xsd: <http://www.w3.org/2001/XMLSchema#> .
      @prefix rdfs: <http://www.w3.org/2000/01/rdf-schema#> .
      @prefix data_ontology: <http://ontosoft.isi.edu:8080/wings-portal/export/users/tirth/TestingDomain/data/ontology.owl#> .

      <http://ontosoft.isi.edu:8080/wings-portal/export/users/tirth/TestingDomain/executions/abstractTest1-83-7336709c-6108-4fc8-9ecd-810f27c8d870.owl#InputFile_html_or_xml>
            a workflow:DataVariable, data_ontology:HTMLfile ;
        rdfs:comment 
          \"center:x=160.701757144928,y=30.331192016601562\"^^xsd:string ;
        workflow:hasDataBinding 
          <http://ontosoft.isi.edu:8080/wings-portal/export/users/tirth/TestingDomain/data/library.owl#test1.html> ;
        workflow:derivedFrom 
          lt;http://ontosoft.isi.edu:8080/wings-portal/export/users/tirth/TestingDomain/workflows/abstractTest1.owl#InputFile_html_or_xml> ;
        data_ontology:hasLanguage 
          \"english\"^^xsd:string ;
        data_ontology:hasSize 
          4 ;
        data_ontology:hasTopic 
          \"basic\"^^xsd:string .
    """^^xsd:string .


###  http://www.wings-workflows.org/ontology/workflow.owl#hasDestinationNode
:hasDestinationNode rdf:type owl:ObjectProperty ,
                             owl:FunctionalProperty ;
                    rdfs:domain :Link ;
                    rdfs:range :Node ;
                    rdfs:comment "The WINGS hasDestinationNode is a WINGS workflow object property that represents a connection between a WingsWorkflow Link and Node i.e. a WingsWorkflowLink hasDestinationNode a WingsWorkflowNode."^^xsd:string ;
                    rdfs:label "hasDestinationNode"^^xsd:string ;
                    <http://www.w3.org/2004/02/skos/core#example> """
        @prefix workflow: <http://www.wings-workflows.org/ontology/workflow.owl#> .

        <http://ontosoft.isi.edu:8080/wings-portal/export/users/tirth/TestingDomain/workflows/
        s6.owl#third_node_InputFile_input>
              a workflow:InputLink ;
          workflow:hasDestinationNode 
            <http://ontosoft.isi.edu:8080/wings-portal/export/users/tirth/TestingDomain/workflows/s6.owl#third_node> ;
          workflow:hasDestinationPort 
            <http://ontosoft.isi.edu:8080/wings-portal/export/users/tirth/TestingDomain/workflows/s6.owl#third_node_InputFile> ;
          workflow:hasVariable 
            <http://ontosoft.isi.edu:8080/wings-portal/export/users/tirth/TestingDomain/workflows/s6.owl#InputFile> .
   """^^xsd:string .


###  http://www.wings-workflows.org/ontology/workflow.owl#hasDestinationPort
:hasDestinationPort rdf:type owl:ObjectProperty ,
                             owl:FunctionalProperty ;
                    rdfs:domain :Link ;
                    rdfs:range :Port ;
                    rdfs:comment "The WINGS hasDestinationPort is a WINGS workflow object property that represents a connection between a WingsWorkflowLink and Port i.e. a WingsWorkflowLink hasDestinationPort WingsWorkflowPort."^^xsd:string ;
                    rdfs:label "hasDestinationPort"^^xsd:string ;
                    <http://www.w3.org/2004/02/skos/core#example> """
        @prefix workflow: <http://www.wings-workflows.org/ontology/workflow.owl#> .

        <http://ontosoft.isi.edu:8080/wings-portal/export/users/tirth/TestingDomain/workflows/
        s6.owl#third_node_InputFile_input>
              a workflow:InputLink ;
          workflow:hasDestinationNode 
            <http://ontosoft.isi.edu:8080/wings-portal/export/users/tirth/TestingDomain/workflows/s6.owl#third_node> ;
          workflow:hasDestinationPort 
            <http://ontosoft.isi.edu:8080/wings-portal/export/users/tirth/TestingDomain/workflows/s6.owl#third_node_InputFile> ;
          workflow:hasVariable 
            <http://ontosoft.isi.edu:8080/wings-portal/export/users/tirth/TestingDomain/workflows/s6.owl#InputFile> .
   """^^xsd:string .


###  http://www.wings-workflows.org/ontology/workflow.owl#hasExpressionArgument
:hasExpressionArgument rdf:type owl:ObjectProperty ;
                       rdfs:domain :SetCreationExpression ;
                       rdfs:range [ rdf:type owl:Class ;
                                    owl:unionOf ( :Port
                                                  :SetCreationExpression
                                                )
                                  ] ;
                       rdfs:comment "The WINGS hasExpressionArgument is a WINGS workflow object property that represents a connection between a SetCreationExpressio and Port."^^xsd:string ;
                       rdfs:label "hasExpressionArgument"^^xsd:string ;
                       <http://www.w3.org/2004/02/skos/core#example> """
      @prefix workflow: <http://www.wings-workflows.org/ontology/workflow.owl#> .

      <http://ontosoft.isi.edu:8080/wings-portal/export/users/tirth/TestingDomain/workflows/s6.owl#_xprod-65d100d0-5360-45a5-a66a-43bf1e7116c9>
            a workflow:XProduct ;
        workflow:hasExpressionArgument 
          <http://ontosoft.isi.edu:8080/wings-portal/export/users/tirth/TestingDomain/workflows/s6.owl#third_node_SecondInputFile>, <http://ontosoft.isi.edu:8080/wings-portal/export/users/tirth/TestingDomain/workflows/s6.owl#third_node_InputFile>, <http://ontosoft.isi.edu:8080/wings-portal/export/users/tirth/TestingDomain/workflows/s6.owl#third_node_InputWord> .
"""^^xsd:string .


###  http://www.wings-workflows.org/ontology/workflow.owl#hasInputPort
:hasInputPort rdf:type owl:ObjectProperty ;
              rdfs:domain :Node ;
              rdfs:range :Port ;
              rdfs:comment "The WINGS hasInputPort is a WINGS workflow object property that represents a connection between a WingsWorkflowNode and Port i.e. a WingsWorkflowNode hasInputPort WingsWorkflowPort."^^xsd:string ;
              rdfs:label "hasInputPort"^^xsd:string ;
              <http://www.w3.org/2004/02/skos/core#example> """
        @prefix workflow: <http://www.wings-workflows.org/ontology/workflow.owl#> .

        <http://ontosoft.isi.edu:8080/wings-portal/export/users/tirth/TestingDomain/workflows/s6.owl#third_node>
              a workflow:Node ;
          rdfs:comment 
            \"center:x=314,y=148\"^^xsd:string ;
          workflow:hasComponent 
            <http://ontosoft.isi.edu:8080/wings-portal/export/users/tirth/TestingDomain/workflows/s6.owl#third_node_comp> ;
          workflow:hasComponentSetCreationRule 
            <http://ontosoft.isi.edu:8080/wings-portal/export/users/tirth/TestingDomain/workflows/s6.owl#third_node_crule> ;
          workflow:hasInputPort 
            <http://ontosoft.isi.edu:8080/wings-portal/export/users/tirth/TestingDomain/workflows/s6.owl#third_node_SecondInputFile>, <http://ontosoft.isi.edu:8080/wings-portal/export/users/tirth/TestingDomain/workflows/s6.owl#third_node_InputFile>, <http://ontosoft.isi.edu:8080/wings-portal/export/users/tirth/TestingDomain/workflows/s6.owl#third_node_InputWord> ;

    """^^xsd:string .


###  http://www.wings-workflows.org/ontology/workflow.owl#hasInputRole
:hasInputRole rdf:type owl:ObjectProperty ;
              rdfs:domain :Workflow ;
              rdfs:range :Role ;
              rdfs:comment "The WINGS hasInputRole is a WINGS workflow object property that represents a connection between a WingsWorkflow SetCreationExpression and Port."^^xsd:string ;
              rdfs:label "hasInputRole"^^xsd:string ;
              <http://www.w3.org/2004/02/skos/core#example> """

      @prefix workflow: <http://www.wings-workflows.org/ontology/workflow.owl#> .

      <http://ontosoft.isi.edu:8080/wings-portal/export/users/tirth/TestingDomain/workflows/r1.owl#r1>
            a workflow:WorkflowTemplate ;
        workflow:hasInputRole 
          <http://ontosoft.isi.edu:8080/wings-portal/export/users/
          tirth/TestingDomain/workflows/r1.owl#InputFormattedFile_irole> ;
        workflow:hasLink 
          <http://ontosoft.isi.edu:8080/wings-portal/export/users/tirth/
          TestingDomain/workflows/r1.owl#xmltotext_node_OutputTextFile_output>,
      
      <http://ontosoft.isi.edu:8080/wings-portal/export/users/tirth/TestingDomain/workflows/r1.owl#xmltotext_node_InputFormattedFile_input> ;
          workflow:hasMetadata 
            <http://ontosoft.isi.edu:8080/wings-portal/export/users/tirth
            /TestingDomain/workflows/r1.owl#r1_meta> ;
          workflow:hasNode 
            <http://ontosoft.isi.edu:8080/wings-portal/export/
            users/tirth/TestingDomain/workflows/r1.owl#xmltotext_node> ;
          workflow:hasOutputRole 
            <http://ontosoft.isi.edu:8080/wings-portal/
            export/users/tirth/TestingDomain/workflows/r1.owl#OutputTextFile_orole> ;
          workflow:hasVersion 
            3 .

   """^^xsd:string .


###  http://www.wings-workflows.org/ontology/workflow.owl#hasLink
:hasLink rdf:type owl:ObjectProperty ;
         rdfs:domain :Workflow ;
         rdfs:range :Link ;
         rdfs:comment "The WINGS hasLink is a WINGS workflow object property that represents a connection between a WingsWorkflow and Link i.e. a WingsWorkflow hasLink WingsWorkflowLink."^^xsd:string ;
         rdfs:label "hasLink"^^xsd:string ;
         <http://www.w3.org/2004/02/skos/core#example> """
      @prefix workflow: <http://www.wings-workflows.org/ontology/workflow.owl#> .

      <http://ontosoft.isi.edu:8080/wings-portal/export/users/tirth/TestingDomain/workflows/s6.owl#s6>
            a <http://www.wings-workflows.org/ontology/workflow.owl#WorkflowTemplate> ;
        workflow:hasInputRole 
          <http://ontosoft.isi.edu:8080/wings-portal/export/users/tirth/TestingDomain/workflows/s6.owl#InputFile_irole>, <http://ontosoft.isi.edu:8080/wings-portal/export/users/tirth/TestingDomain/workflows/s6.owl#InputWord_irole>, <http://ontosoft.isi.edu:8080/wings-portal/export/users/tirth/TestingDomain/workflows/s6.owl#SecondInputFile_irole> ;
        workflow:hasLink 
          <http://ontosoft.isi.edu:8080/wings-portal/export/users/tirth/TestingDomain/workflows/s6.owl#third_node_InputFile_input>, <http://ontosoft.isi.edu:8080/wings-portal/export/users/tirth/TestingDomain/workflows/s6.owl#third_node_SecondInputFile_input>, <http://ontosoft.isi.edu:8080/wings-portal/export/users/tirth/TestingDomain/workflows/s6.owl#third_node_InputWord_input>, <http://ontosoft.isi.edu:8080/wings-portal/export/users/tirth/TestingDomain/workflows/s6.owl#third_node_OutputFile_output> ;
        workflow:hasMetadata 
          <http://ontosoft.isi.edu:8080/wings-portal/export/users/tirth/TestingDomain/workflows/s6.owl#s6_meta> ;
        workflow:hasNode 
          <http://ontosoft.isi.edu:8080/wings-portal/export/users/tirth/TestingDomain/workflows/s6.owl#third_node> ;
        workflow:hasOutputRole 
          <http://ontosoft.isi.edu:8080/wings-portal/export/users/tirth/TestingDomain/workflows/s6.owl#OutputFile_orole> ;
        workflow:hasVersion 
          3 .
    """^^xsd:string .


###  http://www.wings-workflows.org/ontology/workflow.owl#hasMetadata
:hasMetadata rdf:type owl:ObjectProperty ;
             rdfs:domain :Workflow ;
             rdfs:range :Metadata ;
             rdfs:comment "The WINGS hasMetadata is a WINGS workflow object property that represents a connection between a WingsWorkflow and MetaData i.e. a WingsWorkflow hasMetadata WingsWorkflowMetaData."^^xsd:string ;
             rdfs:label "hasMetadata"^^xsd:string ;
             <http://www.w3.org/2004/02/skos/core#example> """
      @prefix workflow: <http://www.wings-workflows.org/ontology/workflow.owl#> .

      <http://ontosoft.isi.edu:8080/wings-portal/export/users/tirth/TestingDomain/workflows/s6.owl#s6>
            a <http://www.wings-workflows.org/ontology/workflow.owl#WorkflowTemplate> ;
        workflow:hasInputRole 
          <http://ontosoft.isi.edu:8080/wings-portal/export/users/tirth/TestingDomain/workflows/s6.owl#InputFile_irole>, <http://ontosoft.isi.edu:8080/wings-portal/export/users/tirth/TestingDomain/workflows/s6.owl#InputWord_irole>, <http://ontosoft.isi.edu:8080/wings-portal/export/users/tirth/TestingDomain/workflows/s6.owl#SecondInputFile_irole> ;
        workflow:hasLink 
          <http://ontosoft.isi.edu:8080/wings-portal/export/users/tirth/TestingDomain/workflows/s6.owl#third_node_InputFile_input>, <http://ontosoft.isi.edu:8080/wings-portal/export/users/tirth/TestingDomain/workflows/s6.owl#third_node_SecondInputFile_input>, <http://ontosoft.isi.edu:8080/wings-portal/export/users/tirth/TestingDomain/workflows/s6.owl#third_node_InputWord_input>, <http://ontosoft.isi.edu:8080/wings-portal/export/users/tirth/TestingDomain/workflows/s6.owl#third_node_OutputFile_output> ;
        workflow:hasMetadata 
          <http://ontosoft.isi.edu:8080/wings-portal/export/users/tirth/TestingDomain/workflows/s6.owl#s6_meta> ;

    """^^xsd:string .


###  http://www.wings-workflows.org/ontology/workflow.owl#hasNode
:hasNode rdf:type owl:ObjectProperty ;
         rdfs:domain :Workflow ;
         rdfs:range :Node ;
         rdfs:comment "The WINGS hasNode is a WINGS workflow object property that represents a connection between a WingsWorkflow and Node i.e. a WingsWorkflow hasNode WingsWorkflowNode."^^xsd:string ;
         rdfs:label "hasNode"^^xsd:string ;
         <http://www.w3.org/2004/02/skos/core#example> """
      @prefix workflow: <http://www.wings-workflows.org/ontology/workflow.owl#> .

      <http://ontosoft.isi.edu:8080/wings-portal/export/users/tirth/TestingDomain/workflows/s6.owl#s6>
            a <http://www.wings-workflows.org/ontology/workflow.owl#WorkflowTemplate> ;
        workflow:hasInputRole 
          <http://ontosoft.isi.edu:8080/wings-portal/export/users/tirth/TestingDomain/workflows/s6.owl#InputFile_irole>, <http://ontosoft.isi.edu:8080/wings-portal/export/users/tirth/TestingDomain/workflows/s6.owl#InputWord_irole>, <http://ontosoft.isi.edu:8080/wings-portal/export/users/tirth/TestingDomain/workflows/s6.owl#SecondInputFile_irole> ;
        workflow:hasLink 
          <http://ontosoft.isi.edu:8080/wings-portal/export/users/tirth/TestingDomain/workflows/s6.owl#third_node_InputFile_input>, <http://ontosoft.isi.edu:8080/wings-portal/export/users/tirth/TestingDomain/workflows/s6.owl#third_node_SecondInputFile_input>, <http://ontosoft.isi.edu:8080/wings-portal/export/users/tirth/TestingDomain/workflows/s6.owl#third_node_InputWord_input>, <http://ontosoft.isi.edu:8080/wings-portal/export/users/tirth/TestingDomain/workflows/s6.owl#third_node_OutputFile_output> ;
        workflow:hasMetadata 
          <http://ontosoft.isi.edu:8080/wings-portal/export/users/tirth/TestingDomain/workflows/s6.owl#s6_meta> ;
        workflow:hasNode 
          <http://ontosoft.isi.edu:8080/wings-portal/export/users/tirth/TestingDomain/workflows/s6.owl#third_node> ;

    """^^xsd:string .


###  http://www.wings-workflows.org/ontology/workflow.owl#hasOriginNode
:hasOriginNode rdf:type owl:ObjectProperty ,
                        owl:FunctionalProperty ;
               rdfs:domain :Link ;
               rdfs:range :Node ;
               rdfs:comment "The WINGS hasOriginNode is a WINGS workflow object property that represents a connection between a WingsWorkflow Link and Node i.e. a WingsWorkflowLink hasOriginNode a WingsWorkflowNode."^^xsd:string ;
               rdfs:label "hasOriginNode"^^xsd:string ;
               <http://www.w3.org/2004/02/skos/core#example> """

  @prefix workflow: <http://www.wings-workflows.org/ontology/workflow.owl#> .

  <http://ontosoft.isi.edu:8080/wings-portal/export/users/
  tirth/TestingDomain/workflows/r1.owl#xmltotext_node_OutputTextFile_output>
        a workflow:OutputLink ;
    workflow:hasOriginNode 
      <http://ontosoft.isi.edu:8080/wings-portal/export/users/
      tirth/TestingDomain/workflows/r1.owl#xmltotext_node> ;
    workflow:hasOriginPort 
      <http://ontosoft.isi.edu:8080/wings-portal/export/users/
      tirth/TestingDomain/workflows/r1.owl#xmltotext_node_OutputTextFile> ;
    workflow:hasVariable 
      <http://ontosoft.isi.edu:8080/wings-portal/export/users/
      tirth/TestingDomain/workflows/r1.owl#OutputTextFile> .
    """^^xsd:string .


###  http://www.wings-workflows.org/ontology/workflow.owl#hasOriginPort
:hasOriginPort rdf:type owl:ObjectProperty ,
                        owl:FunctionalProperty ;
               rdfs:domain :Link ;
               rdfs:range :Port ;
               rdfs:comment "The WINGS hasOriginPort is a WINGS workflow object property that represents a connection between a WingsWorkflowLink and Port i.e. a WingsWorkflowLink hasOriginPort WingsWorkflowPort."^^xsd:string ;
               rdfs:label "hasOriginPort"^^xsd:string ;
               <http://www.w3.org/2004/02/skos/core#example> """

  @prefix workflow: <http://www.wings-workflows.org/ontology/workflow.owl#> .

  <http://ontosoft.isi.edu:8080/wings-portal/export/users/
  tirth/TestingDomain/workflows/r1.owl#xmltotext_node_OutputTextFile_output>
        a workflow:OutputLink ;
    workflow:hasOriginNode 
      <http://ontosoft.isi.edu:8080/wings-portal/export/users/
      tirth/TestingDomain/workflows/r1.owl#xmltotext_node> ;
    workflow:hasOriginPort 
      <http://ontosoft.isi.edu:8080/wings-portal/export/users/
      tirth/TestingDomain/workflows/r1.owl#xmltotext_node_OutputTextFile> ;

   """^^xsd:string .


###  http://www.wings-workflows.org/ontology/workflow.owl#hasOutputPort
:hasOutputPort rdf:type owl:ObjectProperty ;
               rdfs:domain :Node ;
               rdfs:range :Port ;
               rdfs:comment "The WINGS hasOutputPort is a WINGS workflow object property that represents a connection between a WingsWorkflowNode and Port i.e. a WingsWorkflowNode hasOutputPort WingsWorkflowPort."^^xsd:string ;
               rdfs:label "hasOutputPort"^^xsd:string ;
               <http://www.w3.org/2004/02/skos/core#example> """

        @prefix workflow: <http://www.wings-workflows.org/ontology/workflow.owl#> .

        <http://ontosoft.isi.edu:8080/wings-portal/export/users/tirth/TestingDomain/workflows/s6.owl#third_node>
              a workflow:Node ;
          rdfs:comment 
            \"center:x=314,y=148\"^^xsd:string ;
          workflow:hasComponent 
            <http://ontosoft.isi.edu:8080/wings-portal/export/users/tirth/TestingDomain/workflows/s6.owl#third_node_comp> ;
          workflow:hasComponentSetCreationRule 
            <http://ontosoft.isi.edu:8080/wings-portal/export/users/tirth/TestingDomain/workflows/s6.owl#third_node_crule> ;
          workflow:hasInputPort 
            <http://ontosoft.isi.edu:8080/wings-portal/export/users/tirth/TestingDomain/workflows/s6.owl#third_node_SecondInputFile>, <http://ontosoft.isi.edu:8080/wings-portal/export/users/tirth/TestingDomain/workflows/s6.owl#third_node_InputFile>, <http://ontosoft.isi.edu:8080/wings-portal/export/users/tirth/TestingDomain/workflows/s6.owl#third_node_InputWord> ;
          workflow:hasOutputPort 
            <http://ontosoft.isi.edu:8080/wings-portal/export/users/tirth/TestingDomain/workflows/s6.owl#third_node_OutputFile> ;

   """^^xsd:string .


###  http://www.wings-workflows.org/ontology/workflow.owl#hasOutputRole
:hasOutputRole rdf:type owl:ObjectProperty ;
               rdfs:domain :Workflow ;
               rdfs:range :Role ;
               rdfs:comment "The WINGS hasOutputRole is a WINGS workflow object property that represents a connection between a WingsWorkflow and Role i.e. a WingsWorkflow hasOutputRole WingsWorkflowRole."^^xsd:string ;
               rdfs:label "hasOutputRole"^^xsd:string ;
               <http://www.w3.org/2004/02/skos/core#example> """
      @prefix workflow: <http://www.wings-workflows.org/ontology/workflow.owl#> .

      <http://ontosoft.isi.edu:8080/wings-portal/export/users/tirth/TestingDomain/workflows/s6.owl#s6>
            a <http://www.wings-workflows.org/ontology/workflow.owl#WorkflowTemplate> ;
        workflow:hasInputRole 
          <http://ontosoft.isi.edu:8080/wings-portal/export/users/tirth/TestingDomain/workflows/s6.owl#InputFile_irole>, <http://ontosoft.isi.edu:8080/wings-portal/export/users/tirth/TestingDomain/workflows/s6.owl#InputWord_irole>, <http://ontosoft.isi.edu:8080/wings-portal/export/users/tirth/TestingDomain/workflows/s6.owl#SecondInputFile_irole> ;
        workflow:hasLink 
          <http://ontosoft.isi.edu:8080/wings-portal/export/users/tirth/TestingDomain/workflows/s6.owl#third_node_InputFile_input>, <http://ontosoft.isi.edu:8080/wings-portal/export/users/tirth/TestingDomain/workflows/s6.owl#third_node_SecondInputFile_input>, <http://ontosoft.isi.edu:8080/wings-portal/export/users/tirth/TestingDomain/workflows/s6.owl#third_node_InputWord_input>, <http://ontosoft.isi.edu:8080/wings-portal/export/users/tirth/TestingDomain/workflows/s6.owl#third_node_OutputFile_output> ;
        workflow:hasMetadata 
          <http://ontosoft.isi.edu:8080/wings-portal/export/users/tirth/TestingDomain/workflows/s6.owl#s6_meta> ;
        workflow:hasNode 
          <http://ontosoft.isi.edu:8080/wings-portal/export/users/tirth/TestingDomain/workflows/s6.owl#third_node> ;
        workflow:hasOutputRole 
          <http://ontosoft.isi.edu:8080/wings-portal/export/users/tirth/TestingDomain/workflows/s6.owl#OutputFile_orole> ;
    """^^xsd:string .


###  http://www.wings-workflows.org/ontology/workflow.owl#hasPortSetCreationRule
:hasPortSetCreationRule rdf:type owl:ObjectProperty ;
                        rdfs:domain :Node ;
                        rdfs:range :SetCreationRule ;
                        rdfs:comment "The WINGS hasPortSetCreationRule is a WINGS workflow object property that represents a connection between a WingsWorkflowNode and SetCreationRule i.e. a WingsWorkflowNode hasPortSetCreationRule WingsWorkflowSetCreationRule."^^xsd:string ;
                        rdfs:label "hasPortSetCreationRule"^^xsd:string ;
                        <http://www.w3.org/2004/02/skos/core#example> """

        @prefix workflow: <http://www.wings-workflows.org/ontology/workflow.owl#> .

        <http://ontosoft.isi.edu:8080/wings-portal/export/users/tirth/TestingDomain/workflows/s6.owl#third_node>
              a workflow:Node ;
          rdfs:comment 
            \"center:x=314,y=148\"^^xsd:string ;
          workflow:hasComponent 
            <http://ontosoft.isi.edu:8080/wings-portal/export/users/tirth/TestingDomain/workflows/s6.owl#third_node_comp> ;
          workflow:hasComponentSetCreationRule 
            <http://ontosoft.isi.edu:8080/wings-portal/export/users/tirth/TestingDomain/workflows/s6.owl#third_node_crule> ;
          workflow:hasInputPort 
            <http://ontosoft.isi.edu:8080/wings-portal/export/users/tirth/TestingDomain/workflows/s6.owl#third_node_SecondInputFile>, <http://ontosoft.isi.edu:8080/wings-portal/export/users/tirth/TestingDomain/workflows/s6.owl#third_node_InputFile>, <http://ontosoft.isi.edu:8080/wings-portal/export/users/tirth/TestingDomain/workflows/s6.owl#third_node_InputWord> ;
          workflow:hasOutputPort 
            <http://ontosoft.isi.edu:8080/wings-portal/export/users/tirth/TestingDomain/workflows/s6.owl#third_node_OutputFile> ;
          workflow:hasPortSetCreationRule 
            <http://ontosoft.isi.edu:8080/wings-portal/export/users/tirth/TestingDomain/workflows/s6.owl#third_node_prule> .

   """^^xsd:string .


###  http://www.wings-workflows.org/ontology/workflow.owl#hasVariable
:hasVariable rdf:type owl:ObjectProperty ,
                      owl:FunctionalProperty ;
             rdfs:domain :Link ;
             rdfs:range :Variable ;
             rdfs:comment "The WINGS hasVariable is a WINGS workflow object property that represents a connection between a WingsWorkflow Link and Variable i.e. a WingsWorkflowLink hasVariable a WingsWorkflowVariable."^^xsd:string ;
             rdfs:label "hasVariable"^^xsd:string ;
             <http://www.w3.org/2004/02/skos/core#example> """

  @prefix workflow: <http://www.wings-workflows.org/ontology/workflow.owl#> .

  <http://ontosoft.isi.edu:8080/wings-portal/export/users/
  tirth/TestingDomain/workflows/r1.owl#xmltotext_node_OutputTextFile_output>
        a workflow:OutputLink ;
    workflow:hasOriginNode 
      <http://ontosoft.isi.edu:8080/wings-portal/export/users/
      tirth/TestingDomain/workflows/r1.owl#xmltotext_node> ;
    workflow:hasOriginPort 
      <http://ontosoft.isi.edu:8080/wings-portal/export/users/
      tirth/TestingDomain/workflows/r1.owl#xmltotext_node_OutputTextFile> ;
    workflow:hasVariable 
      <http://ontosoft.isi.edu:8080/wings-portal/export/users/
      tirth/TestingDomain/workflows/r1.owl#OutputTextFile> .

   """^^xsd:string .


###  http://www.wings-workflows.org/ontology/workflow.owl#hasWorkflow
:hasWorkflow rdf:type owl:ObjectProperty ;
             rdfs:domain :Node ;
             rdfs:range :Workflow ;
             rdfs:comment "The WINGS hasWorkflow is a WINGS workflow object property that represents a connection between a WingsWorkflow Node and WingsWorkflow i.e. a WingsWorkflowNode hasWorkflow WingsWorkflow."^^xsd:string ;
             rdfs:label "hasWorkflow"^^xsd:string .


###  http://www.wings-workflows.org/ontology/workflow.owl#mapsToVariable
:mapsToVariable rdf:type owl:ObjectProperty ;
                rdfs:domain :Role ;
                rdfs:range :Variable ;
                rdfs:comment "The WINGS mapsToVariable is a WINGS workflow object property that represents a connection between a WingsWorkflow Role and WingsWorkflowVariable i.e. a WingsWorkflowNRole mapsToVariable WingsWorkflowVariable."^^xsd:string ;
                rdfs:label "mapsToVariable"^^xsd:string ;
                <http://www.w3.org/2004/02/skos/core#example> """
      @prefix workflow: <http://www.wings-workflows.org/ontology/workflow.owl#> .

      <http://ontosoft.isi.edu:8080/wings-portal/export/users/tirth/TestingDomain/workflows/s6.owl#InputFile_irole>
            a workflow:Role ;
        workflow:mapsToVariable 
          <http://ontosoft.isi.edu:8080/wings-portal/export/users/tirth/TestingDomain/workflows/s6.owl#InputFile> ;
        workflow:hasRoleID 
          \"third_node_InputFile\"^^xsd:string ;
        workflow:hasDimensionality 
          0 .
    """^^xsd:string .


###  http://www.wings-workflows.org/ontology/workflow.owl#satisfiesRole
:satisfiesRole rdf:type owl:ObjectProperty ;
               rdfs:domain :Port ;
               rdfs:range :Role ;
               rdfs:comment "The WINGS satisfiesRole is a WINGS workflow object property that represents a connection between a WingsWorkflowPort and WingsWorkflowRole i.e. a WingsWorkflowPort satisfiesRole WingsWorkflowRole."^^xsd:string ;
               rdfs:label "satisfiesRole"^^xsd:string ;
               <http://www.w3.org/2004/02/skos/core#example> """

  @prefix workflow: <http://www.wings-workflows.org/ontology/workflow.owl#> .

  <http://ontosoft.isi.edu:8080/wings-portal/export/users/tirth/TestingDomain/workflows/r1.owl#xmltotext_node_InputFormattedFile>
        a workflow:Port ;
    workflow:satisfiesRole 
      <http://ontosoft.isi.edu:8080/wings-portal/export/users/
      tirth/TestingDomain/workflows/r1.owl#xmltotext_node_InputFormattedFile_role> .

    """^^xsd:string .


#################################################################
#    Data properties
#################################################################

###  http://www.wings-workflows.org/ontology/workflow.owl#autoFill
:autoFill rdf:type owl:DatatypeProperty ;
          rdfs:domain :ParameterVariable ;
          rdfs:range xsd:boolean ;
          rdfs:comment "The WINGS autoFill is a WINGS workflow data property that represents a WingsWorkflowParameterVariable is autoFillable or not (specified as a boolean)."^^xsd:string ;
          rdfs:label "autoFill"^^xsd:string .


###  http://www.wings-workflows.org/ontology/workflow.owl#breakPoint
:breakPoint rdf:type owl:DatatypeProperty .


###  http://www.wings-workflows.org/ontology/workflow.owl#createComponentSets
:createComponentSets rdf:type owl:DatatypeProperty ;
                     rdfs:domain :SetCreationRule ;
                     rdfs:range xsd:boolean ;
                     rdfs:comment "The WINGS createComponentSets is a WINGS workflow data property that represents a WingsWorkflowSetCreationRule has the ability to createComponentSets."^^xsd:string ;
                     rdfs:label "createComponentSets"^^xsd:string ;
                     <http://www.w3.org/2004/02/skos/core#example> """
      @prefix workflow: <http://www.wings-workflows.org/ontology/workflow.owl#> .

      <http://ontosoft.isi.edu:8080/wings-portal/export/users/tirth/TestingDomain/workflows/s6.owl#third_node_prule>
            a workflow:PortSetRule ;
        workflow:createSetsOn 
          <http://ontosoft.isi.edu:8080/wings-portal/export/users/tirth/TestingDomain/workflows/s6.owl#_xprod-65d100d0-5360-45a5-a66a-43bf1e7116c9> ;
        workflow:createComponentSets 
          true .
    """^^xsd:string .


###  http://www.wings-workflows.org/ontology/workflow.owl#createWorkflowSets
:createWorkflowSets rdf:type owl:DatatypeProperty ;
                    rdfs:domain :SetCreationRule ;
                    rdfs:range xsd:boolean ;
                    rdfs:comment "The WINGS createWorkflowSets is a WINGS workflow data property that represents a WingsWorkflowSetCreationRule has the ability to createWorkflowSets."^^xsd:string ;
                    rdfs:label "createWorkflowSets"^^xsd:string ;
                    <http://www.w3.org/2004/02/skos/core#example> """

      @prefix workflow: <http://www.wings-workflows.org/ontology/workflow.owl#> .

      <http://ontosoft.isi.edu:8080/wings-portal/export/users/tirth/TestingDomain/workflows/s6.owl#third_node_crule>
            a workflow:ComponentSetRule ;
      workflow:createSetsOn 
        <http://ontosoft.isi.edu:8080/wings-portal/export/users/tirth/TestingDomain/workflows/s6.owl#third_node_comp> ;
      workflow:createWorkflowSets 
        true .

    """^^xsd:string .


###  http://www.wings-workflows.org/ontology/workflow.owl#createdFrom
:createdFrom rdf:type owl:DatatypeProperty ;
             rdfs:domain :Metadata ;
             rdfs:range xsd:string ;
             rdfs:comment "The WINGS createdFrom is a WINGS workflow data property that represents the WingsWorkflowMetaData has createdFrom as a property."^^xsd:string ;
             rdfs:label "createdFrom"^^xsd:string .


###  http://www.wings-workflows.org/ontology/workflow.owl#hasContributor
:hasContributor rdf:type owl:DatatypeProperty ;
                rdfs:domain :Metadata ;
                rdfs:range xsd:string ;
                rdfs:comment "The WINGS hasContributor is a WINGS workflow data property that represents a WingsWorkflow has a contributor (specified as a string)."^^xsd:string ;
                rdfs:label "hasContributor"^^xsd:string ;
                <http://www.w3.org/2004/02/skos/core#example> """

    @prefix workflow: <http://www.wings-workflows.org/ontology/workflow.owl#> .
    @prefix xsd: <http://www.w3.org/2001/XMLSchema#> .

    <http://ontosoft.isi.edu:8080/wings-portal/export/users/
    tirth/TestingDomain/workflows/r1.owl#r1_meta>
        a workflow:Metadata ;
      workflow:hasContributor
        \"tirth\"^^xsd:string ;
      workflow:lastUpdateTime
        \"2017-07-14T07:00:00Z\"^^xsd:dateTime .

    """^^xsd:string .


###  http://www.wings-workflows.org/ontology/workflow.owl#hasDimensionality
:hasDimensionality rdf:type owl:DatatypeProperty ,
                            owl:FunctionalProperty ;
                   rdfs:range xsd:int ;
                   rdfs:comment """The WINGS hasDimensionality is a WINGS workflow data property that represents a WingsWorkflow Input is a collection or not (specified as a number(int)).
    """^^xsd:string ;
                   rdfs:label "hasDimensionality"^^xsd:string ;
                   <http://www.w3.org/2004/02/skos/core#example> """

      @prefix workflow: <http://www.wings-workflows.org/ontology/workflow.owl#> .
      @prefix xsd: <http://www.w3.org/2001/XMLSchema#> .
      @prefix rdfs: <http://www.w3.org/2000/01/rdf-schema#> .
      @prefix data_ontology: <http://ontosoft.isi.edu:8080/wings-portal/export/users/tirth/TestingDomain/data/ontology.owl#> .

      <http://ontosoft.isi.edu:8080/wings-portal/export/users/tirth/TestingDomain/workflows/s6.owl#InputFile_irole>
            a workflow:Role ;
        workflow:mapsToVariable 
          <http://ontosoft.isi.edu:8080/wings-portal/export/users/tirth/TestingDomain/workflows/s6.owl#InputFile> ;
        workflow:hasRoleID 
          \"third_node_InputFile\"^^xsd:string ;
        workflow:hasDimensionality 
          0 .

    """^^xsd:string .


###  http://www.wings-workflows.org/ontology/workflow.owl#hasDocumentation
:hasDocumentation rdf:type owl:DatatypeProperty ;
                  rdfs:domain :Metadata ;
                  rdfs:range xsd:string ;
                  rdfs:comment "The WINGS hasDocumentation is a WINGS workflow data property that represents a WingsWorkflow metadata contains documentation for the workflow."^^xsd:string ;
                  rdfs:label "hasDocumentation"^^xsd:string .


###  http://www.wings-workflows.org/ontology/workflow.owl#hasParameterValue
:hasParameterValue rdf:type owl:DatatypeProperty ;
                   rdfs:domain :ParameterVariable ;
                   rdfs:comment "The WINGS hasParameterValue is a WINGS workflow data property that represents a WingsWorkflow parameter variable has a parameter value."^^xsd:string ;
                   rdfs:label "hasParameterValue"^^xsd:string ;
                   <http://www.w3.org/2004/02/skos/core#example> """
      @prefix workflow: <http://www.wings-workflows.org/ontology/workflow.owl#> .
      @prefix xsd: <http://www.w3.org/2001/XMLSchema#> .
      @prefix rdfs: <http://www.w3.org/2000/01/rdf-schema#> .
      @prefix data_ontology: <http://ontosoft.isi.edu:8080/wings-portal/export/users/tirth/TestingDomain/data/ontology.owl#> .

      <http://ontosoft.isi.edu:8080/wings-portal/export/users/tirth/TestingDomain/executions/abstractTest1-83-7336709c-6108-4fc8-9ecd-810f27c8d870.owl#WordInput>
            a workflow:ParameterVariable ;
        rdfs:comment 
          \"center:x=366.40000000000003,y=196.99678802490234\"^^xsd:string ;
        workflow:derivedFrom 
          <http://ontosoft.isi.edu:8080/wings-portal/export/users/tirth/TestingDomain/workflows/abstractTest1.owl#WordInput> ;
        workflow:hasParameterValue 
          \"great\"^^xsd:string .
    """^^xsd:string .


###  http://www.wings-workflows.org/ontology/workflow.owl#hasRoleID
:hasRoleID rdf:type owl:DatatypeProperty ;
           rdfs:domain :Role ;
           rdfs:range xsd:string ;
           rdfs:comment "The WINGS hasRoleID is a WINGS workflow data property that represents a WingsWorkflowRole has a role id."^^xsd:string ;
           rdfs:label "hasRoleID"^^xsd:string ;
           <http://www.w3.org/2004/02/skos/core#example> """

           @prefix workflow: <http://www.wings-workflows.org/ontology/workflow.owl#> .

           <http://ontosoft.isi.edu:8080/wings-portal/export/users/
           tirth/TestingDomain/workflows/r1.owl#xmltotext_node_InputFormattedFile_role>
              workflow:hasRoleID 
                \"InputFormattedFile\"^^xsd:string ;
              workflow:hasDimensionality 
                0 .


       """^^xsd:string .


###  http://www.wings-workflows.org/ontology/workflow.owl#hasRules
:hasRules rdf:type owl:DatatypeProperty ;
          rdfs:domain :Workflow ;
          rdfs:range xsd:string ;
          rdfs:comment "The WINGS hasRules is a WINGS workflow data property that represents a WingsWorkflow has a set of rules (specified as strings)."^^xsd:string ;
          rdfs:label "hasRules"^^xsd:string .


###  http://www.wings-workflows.org/ontology/workflow.owl#hasVersion
:hasVersion rdf:type owl:DatatypeProperty ;
            rdfs:domain :Workflow ;
            rdfs:range xsd:int ;
            rdfs:comment "The WINGS hasVersion is a WINGS workflow data property that represents a WingsWorkflow has a version number."^^xsd:string ;
            rdfs:label "hasVersion"^^xsd:string ;
            <http://www.w3.org/2004/02/skos/core#example> """
      @prefix workflow: <http://www.wings-workflows.org/ontology/workflow.owl#> .

      <http://ontosoft.isi.edu:8080/wings-portal/export/users/tirth/TestingDomain/workflows/s6.owl#s6>
            a workflow:WorkflowTemplate ;
        workflow:hasInputRole 
          <http://ontosoft.isi.edu:8080/wings-portal/export/users/tirth/TestingDomain/workflows/s6.owl#InputFile_irole>, <http://ontosoft.isi.edu:8080/wings-portal/export/users/tirth/TestingDomain/workflows/s6.owl#InputWord_irole>, <http://ontosoft.isi.edu:8080/wings-portal/export/users/tirth/TestingDomain/workflows/s6.owl#SecondInputFile_irole> ;
        workflow:hasLink 
          <http://ontosoft.isi.edu:8080/wings-portal/export/users/tirth/TestingDomain/workflows/s6.owl#third_node_InputFile_input>, <http://ontosoft.isi.edu:8080/wings-portal/export/users/tirth/TestingDomain/workflows/s6.owl#third_node_SecondInputFile_input>, <http://ontosoft.isi.edu:8080/wings-portal/export/users/tirth/TestingDomain/workflows/s6.owl#third_node_InputWord_input>, <http://ontosoft.isi.edu:8080/wings-portal/export/users/tirth/TestingDomain/workflows/s6.owl#third_node_OutputFile_output> ;
        workflow:hasMetadata 
          <http://ontosoft.isi.edu:8080/wings-portal/export/users/tirth/TestingDomain/workflows/s6.owl#s6_meta> ;
        workflow:hasNode 
          <http://ontosoft.isi.edu:8080/wings-portal/export/users/tirth/TestingDomain/workflows/s6.owl#third_node> ;
        workflow:hasOutputRole 
          <http://ontosoft.isi.edu:8080/wings-portal/export/users/tirth/TestingDomain/workflows/s6.owl#OutputFile_orole> ;
        workflow:hasVersion 
          3 .
    """^^xsd:string .


###  http://www.wings-workflows.org/ontology/workflow.owl#isConcrete
:isConcrete rdf:type owl:DatatypeProperty ,
                     owl:FunctionalProperty ;
            rdfs:domain :ComponentVariable ;
            rdfs:range xsd:boolean ;
            rdfs:comment "The WINGS isConcrete is a WINGS workflow data property that represents a WingsWorkflow Component Variable is abstract or concrete."^^xsd:string ;
            rdfs:label "isConcrete"^^xsd:string ;
            <http://www.w3.org/2004/02/skos/core#example> """
        @prefix workflow: <http://www.wings-workflows.org/ontology/workflow.owl#> .

        <http://ontosoft.isi.edu:8080/wings-portal/export/users/tirth/TestingDomain/workflows/r1.owl#xmltotext_node_comp>
          workflow:hasComponentBinding
            <http://ontosoft.isi.edu:8080/wings-portal/export/users/tirth/TestingDomain/components/library.owl#xmltotext> ;
          workflow:isConcrete
            true . 

   """^^xsd:string .


###  http://www.wings-workflows.org/ontology/workflow.owl#isInactive
:isInactive rdf:type owl:DatatypeProperty ,
                     owl:FunctionalProperty ;
            rdfs:range xsd:boolean ;
            rdfs:comment "The WINGS isInactive is a WINGS workflow data property that represents a WingsWorkflow is active or not."^^xsd:string ;
            rdfs:label "isInactive"^^xsd:string .


###  http://www.wings-workflows.org/ontology/workflow.owl#lastUpdateTime
:lastUpdateTime rdf:type owl:DatatypeProperty ;
                rdfs:domain :Metadata ;
                rdfs:range xsd:dateTime ;
                rdfs:comment "The WINGS lastUpdateTime is a WINGS workflow data property that represents a WingsWorkflow has a last updated time(the range being a dateTime)."^^xsd:string ;
                rdfs:label "lastUpdateTime"^^xsd:string ;
                <http://www.w3.org/2004/02/skos/core#example> """

    @prefix workflow: <http://www.wings-workflows.org/ontology/workflow.owl#> .
    @prefix xsd: <http://www.w3.org/2001/XMLSchema#> .

    <http://ontosoft.isi.edu:8080/wings-portal/export/users/
    tirth/TestingDomain/workflows/r1.owl#r1_meta>
        a workflow:Metadata ;
      workflow:hasContributor
        \"tirth\"^^xsd:string ;
      workflow:lastUpdateTime
        \"2017-07-14T07:00:00Z\"^^xsd:dateTime .

    """^^xsd:string .


###  http://www.wings-workflows.org/ontology/workflow.owl#tellmeData
:tellmeData rdf:type owl:DatatypeProperty ;
            rdfs:domain :Metadata ;
            rdfs:range xsd:string ;
            rdfs:comment "The WINGS tellmeData is a WINGS workflow data property that represents a WingsWorkflowMetadata has a property for knowing the data (specifying the data as a set of strings)."^^xsd:string ;
            rdfs:label "tellmeData"^^xsd:string .


#################################################################
#    Classes
#################################################################

###  http://www.w3.org/2001/XMLSchema#true
xsd:true rdf:type owl:Class .


###  http://www.wings-workflows.org/ontology/resource.owl#Machine
<http://www.wings-workflows.org/ontology/resource.owl#Machine> rdf:type owl:Class .


###  http://www.wings-workflows.org/ontology/workflow.owl#ComponentSetRule
:ComponentSetRule rdf:type owl:Class ;
                  rdfs:subClassOf :SetCreationRule ;
                  rdfs:comment "The WINGS ComponentSetRule is a WINGS workflow class that represents a set of component rules in the workflow specification."^^xsd:string ;
                  rdfs:label "ComponentSetRule"^^xsd:string ;
                  <http://www.w3.org/2004/02/skos/core#example> """
         @prefix workflow: <http://www.wings-workflows.org/ontology/workflow.owl#> .

         <http://ontosoft.isi.edu:8080/wings-portal/export/users/tirth/TestingDomain/workflows/s6.owl#third_node_crule>
              a workflow:ComponentSetRule ;
            workflow:createSetsOn 
              <http://ontosoft.isi.edu:8080/wings-portal/export/users/tirth/TestingDomain/workflows/s6.owl#third_node_comp> ;
            workflow:createWorkflowSets 
              true .
        """^^xsd:string .


###  http://www.wings-workflows.org/ontology/workflow.owl#ComponentVariable
:ComponentVariable rdf:type owl:Class ;
                   rdfs:subClassOf :Variable ;
                   rdfs:comment "The WINGS ComponentVariable is a WINGS workflow class that represents a component variable in the workflow specification."^^xsd:string ;
                   rdfs:label "ComponentVariable"^^xsd:string .


###  http://www.wings-workflows.org/ontology/workflow.owl#DataVariable
:DataVariable rdf:type owl:Class ;
              rdfs:subClassOf :Variable ;
              rdfs:comment "The WINGS data variable is a WINGS workflow class that represents a workflow template artifact in OPMW and is a variable in the WINGS template specification."^^xsd:string ;
              rdfs:label "DataVariable"^^xsd:string ;
              <http://www.w3.org/2004/02/skos/core#example> """

      @prefix workflow: <http://www.wings-workflows.org/ontology/workflow.owl#> .
      @prefix rdfs: <http://www.w3.org/2000/01/rdf-schema#> .
      @prefix xsd: <http://www.w3.org/2001/XMLSchema#> .

      <http://ontosoft.isi.edu:8080/wings-portal/export/users/
      tirth/TestingDomain/workflows/r1.owl#OutputTextFile>
          a workflow:DataVariable ;
          rdfs:comment \"center:x=214.0035400390625,y=196.80760192871094\"^^xsd:string .

        """^^xsd:string .


###  http://www.wings-workflows.org/ontology/workflow.owl#InOutLink
:InOutLink rdf:type owl:Class ;
           rdfs:subClassOf :Link ;
           rdfs:comment "The WINGS inout link is a WINGS workflow class that has an origin node, a destination node and a variable."^^xsd:string ;
           rdfs:label "InOutLink"^^xsd:string ;
           <http://www.w3.org/2004/02/skos/core#example> """

  @prefix workflow: <http://www.wings-workflows.org/ontology/workflow.owl#> .

  <http://ontosoft.isi.edu:8080/wings-portal/export/users/tirth/TestingDomain/workflows/abstractTest1.owl#ConvertToText_node_OutputTextFile_to_countingWords_node_InputTextFile>
      a workflow:InOutLink ;
    workflow:hasDestinationNode 
        <http://ontosoft.isi.edu:8080/wings-portal/export/users/
        tirth/TestingDomain/workflows/abstractTest1.owl#countingWords_node> ;
    workflow:hasDestinationPort 
        <http://ontosoft.isi.edu:8080/wings-portal/export/users/
        tirth/TestingDomain/workflows/abstractTest1.owl#countingWords_node_InputTextFile> ;
    workflow:hasOriginNode 
        <http://ontosoft.isi.edu:8080/wings-portal/export/users/
        tirth/TestingDomain/workflows/abstractTest1.owl#ConvertToText_node> ;
    workflow:hasOriginPort 
        <http://ontosoft.isi.edu:8080/wings-portal/export/users/
        tirth/TestingDomain/workflows/abstractTest1.owl#ConvertToText_node_OutputTextFile> ;
    workflow:hasVariable 
        <http://ontosoft.isi.edu:8080/wings-portal/export/users/
        tirth/TestingDomain/workflows/abstractTest1.owl#Intermediate_Result> .


        """^^xsd:string .


###  http://www.wings-workflows.org/ontology/workflow.owl#IncreaseDimensionality
:IncreaseDimensionality rdf:type owl:Class ;
                        rdfs:subClassOf :SetCreationExpression .


###  http://www.wings-workflows.org/ontology/workflow.owl#InputLink
:InputLink rdf:type owl:Class ;
           rdfs:subClassOf :Link ;
           rdfs:comment "The WINGS input link is a WINGS workflow class that has a destination node and a variable."^^xsd:string ;
           rdfs:label "InputLink"^^xsd:string ;
           <http://www.w3.org/2004/02/skos/core#example> """

      @prefix workflow: <http://www.wings-workflows.org/ontology/workflow.owl#> .

      <http://ontosoft.isi.edu:8080/wings-portal/export/users/
      tirth/TestingDomain/workflows/r1.owl#xmltotext_node_InputFormattedFile_input>
          a workflow:InputLink ;
        workflow:hasDestinationNode
            <http://ontosoft.isi.edu:8080/wings-portal/export/users/
            tirth/TestingDomain/workflows/r1.owl#xmltotext_node> ;
        workflow:hasDestinationPort
            <http://ontosoft.isi.edu:8080/wings-portal/export/users/
            tirth/TestingDomain/workflows/r1.owl#xmltotext_node_InputFormattedFile> ;
        workflow:hasVariable
            <http://ontosoft.isi.edu:8080/wings-portal/export/users/
            tirth/TestingDomain/workflows/r1.owl#InputFormattedFile> .

       """^^xsd:string .


###  http://www.wings-workflows.org/ontology/workflow.owl#Link
:Link rdf:type owl:Class ;
      rdfs:comment "The WINGS Link is a WINGS workflow class that represents a link in the template specification."^^xsd:string ;
      rdfs:label "Link"^^xsd:string .


###  http://www.wings-workflows.org/ontology/workflow.owl#Metadata
:Metadata rdf:type owl:Class ;
          rdfs:comment "The WINGS MetaData is a WINGS workflow class that represents the metadata pertaining to a template specification."^^xsd:string ;
          rdfs:label "Metadata"^^xsd:string ;
          <http://www.w3.org/2004/02/skos/core#example> """

    @prefix workflow: <http://www.wings-workflows.org/ontology/workflow.owl#> .
    @prefix xsd: <http://www.w3.org/2001/XMLSchema#> .

    <http://ontosoft.isi.edu:8080/wings-portal/export/users/
    tirth/TestingDomain/workflows/r1.owl#r1_meta>
        a workflow:Metadata ;
      workflow:hasContributor
        \"tirth\"^^xsd:string ;
      workflow:lastUpdateTime
        \"2017-07-14T07:00:00Z\"^^xsd:dateTime .

    """^^xsd:string .


###  http://www.wings-workflows.org/ontology/workflow.owl#NWise
:NWise rdf:type owl:Class ;
       rdfs:subClassOf :SetCreationExpression .


###  http://www.wings-workflows.org/ontology/workflow.owl#Node
:Node rdf:type owl:Class ;
      rdfs:comment "The WINGS Node is a WINGS workflow class that represents a node in the template specification. The node has components in templates."^^xsd:string ;
      rdfs:label "Node"^^xsd:string ;
      <http://www.w3.org/2004/02/skos/core#example> """

  @prefix workflow: <http://www.wings-workflows.org/ontology/workflow.owl#> .
  @prefix rdfs: <http://www.w3.org/2000/01/rdf-schema#> .
  @prefix xsd: <http://www.w3.org/2001/XMLSchema#> .

  <http://ontosoft.isi.edu:8080/wings-portal/export/users/
  tirth/TestingDomain/workflows/r1.owl#xmltotext_node>
        a workflow:Node ;
    rdfs:comment
      \"center:x=220,y=130\"^^xsd:string ;
    workflow:hasComponent
      <http://ontosoft.isi.edu:8080/wings-portal/export/users/
      tirth/TestingDomain/workflows/r1.owl#xmltotext_node_comp> ;
    workflow:hasComponentSetCreationRule
      <http://ontosoft.isi.edu:8080/wings-portal/export/users
      tirth/TestingDomain/workflows/r1.owl#xmltotext_node_crule> ;
    workflow:hasInputPort
      <http://ontosoft.isi.edu:8080/wings-portal/export/users/
      tirth/TestingDomain/workflows/r1.owl#xmltotext_node_InputFormattedFile> ;
    workflow:hasOutputPort
      <http://ontosoft.isi.edu:8080/wings-portal/export/users/
      tirth/TestingDomain/workflows/r1.owl#xmltotext_node_OutputTextFile> ;
    workflow:hasPortSetCreationRule 
      <http://ontosoft.isi.edu:8080/wings-portal/export/users/
      tirth/TestingDomain/workflows/r1.owl#xmltotext_node_prule> .

  """^^xsd:string .


###  http://www.wings-workflows.org/ontology/workflow.owl#OutputLink
:OutputLink rdf:type owl:Class ;
            rdfs:subClassOf :Link ;
            rdfs:comment "The WINGS output link is a WINGS workflow class that has an origin node and a variable."^^xsd:string ;
            rdfs:label "OutputLink"^^xsd:string ;
            <http://www.w3.org/2004/02/skos/core#example> """

  @prefix workflow: <http://www.wings-workflows.org/ontology/workflow.owl#> .

  <http://ontosoft.isi.edu:8080/wings-portal/export/users/
  tirth/TestingDomain/workflows/r1.owl#xmltotext_node_OutputTextFile_output>
        a workflow:OutputLink ;
    workflow:hasOriginNode
      <http://ontosoft.isi.edu:8080/wings-portal/export/users/
      tirth/TestingDomain/workflows/r1.owl#xmltotext_node> ;
    workflow:hasOriginPort 
      <http://ontosoft.isi.edu:8080/wings-portal/export/users
      tirth/TestingDomain/workflows/r1.owl#xmltotext_node_OutputTextFile> ;
    workflow:hasVariable
      <http://ontosoft.isi.edu:8080/wings-portal/export/users/
      tirth/TestingDomain/workflows/r1.owl#OutputTextFile> . 

   """^^xsd:string .


###  http://www.wings-workflows.org/ontology/workflow.owl#ParameterVariable
:ParameterVariable rdf:type owl:Class ;
                   rdfs:subClassOf :Variable ;
                   rdfs:comment "A parameter variable is a WINGS workflow class that represents a description of an input parameter of a workflow step."^^xsd:string ;
                   rdfs:label "ParameterVariable"^^xsd:string ;
                   <http://www.w3.org/2004/02/skos/core#example> """

@prefix workflow: <http://www.wings-workflows.org/ontology/workflow.owl#> .
@prefix rdfs: <http://www.w3.org/2000/01/rdf-schema#> .
@prefix xsd: <http://www.w3.org/2001/XMLSchema#> .

<http://ontosoft.isi.edu:8080/wings-portal/export/users/tirth/TestingDomain/workflows/s6.owl#InputWord>
      a workflow:ParameterVariable ;
    rdfs:comment 
      \"center:x=315.0057067871094,y=72.19681549072266\"^^xsd:string .


   """^^xsd:string .


###  http://www.wings-workflows.org/ontology/workflow.owl#Port
:Port rdf:type owl:Class .


###  http://www.wings-workflows.org/ontology/workflow.owl#PortSetRule
:PortSetRule rdf:type owl:Class ;
             rdfs:subClassOf :SetCreationRule ;
             rdfs:label "PortSetRule"^^xsd:string ;
             <http://www.w3.org/2004/02/skos/core#example> """

  @prefix workflow: <http://www.wings-workflows.org/ontology/workflow.owl#> .

  <http://ontosoft.isi.edu:8080/wings-portal/export/users/
  tirth/TestingDomain/workflows/s6.owl#third_node_prule>
        a workflow:PortSetRule ;
    workflow:createSetsOn
      <http://ontosoft.isi.edu:8080/wings-portal/export/users/
      tirth/TestingDomain/workflows/s6.owl#_xprod-65d100d0-5360-45a5-a66a-43bf1e7116c9> ;
    workflow:createComponentSets
      true .

 """^^xsd:string .


###  http://www.wings-workflows.org/ontology/workflow.owl#ReduceDimensionality
:ReduceDimensionality rdf:type owl:Class ;
                      rdfs:subClassOf :SetCreationExpression .


###  http://www.wings-workflows.org/ontology/workflow.owl#Role
:Role rdf:type owl:Class .


###  http://www.wings-workflows.org/ontology/workflow.owl#SetCreationExpression
:SetCreationExpression rdf:type owl:Class .


###  http://www.wings-workflows.org/ontology/workflow.owl#SetCreationRule
:SetCreationRule rdf:type owl:Class .


###  http://www.wings-workflows.org/ontology/workflow.owl#Shift
:Shift rdf:type owl:Class ;
       rdfs:subClassOf :SetCreationExpression .


###  http://www.wings-workflows.org/ontology/workflow.owl#Variable
:Variable rdf:type owl:Class ;
          rdfs:label "Variable"^^xsd:string ;
          <http://www.w3.org/2004/02/skos/core#example> """


@prefix workflow: <http://www.wings-workflows.org/ontology/workflow.owl#> .
@prefix xsd: <http://www.w3.org/2001/XMLSchema#> .

<http://ontosoft.isi.edu:8080/wings-portal/export/users/tirth/TestingDomain/workflows/s6.owl#InputWord>
        a workflow:ParameterVariable ;
    rdfs:comment
      \"center:x=315.0057067871094,y=72.19681549072266\"^^xsd:string .

   """^^xsd:string .


###  http://www.wings-workflows.org/ontology/workflow.owl#Workflow
:Workflow rdf:type owl:Class ;
          rdfs:comment "The WINGS workflow is a class in the WINGS Ontology that represents the entire workflow created in the WINGS workflow system."^^xsd:string ;
          rdfs:label "Workflow"^^xsd:string .


###  http://www.wings-workflows.org/ontology/workflow.owl#WorkflowInstance
:WorkflowInstance rdf:type owl:Class ;
                  rdfs:subClassOf :Workflow ;
                  rdfs:comment "The WINGS WorkflowInstance is a class in the WINGS Ontology that represents the workflow instance that is connected to a workflow execution file by the relation hasPlan workflowInstance."^^xsd:string ;
                  rdfs:label "WorkflowInstance"^^xsd:string .


###  http://www.wings-workflows.org/ontology/workflow.owl#WorkflowTemplate
:WorkflowTemplate rdf:type owl:Class ;
                  rdfs:subClassOf :Workflow ;
                  rdfs:comment "The WINGS workflow template is a class in the WINGS Ontology that represents the entire workflow template created in the WINGS workflow system."^^xsd:string ;
                  rdfs:label "WorkflowTemplate"^^xsd:string ;
                  <http://www.w3.org/2004/02/skos/core#example> """

  @prefix workflow: <http://www.wings-workflows.org/ontology/workflow.owl#> .
  
  <http://ontosoft.isi.edu:8080/wings-portal/export/users/
  tirth/TestingDomain/workflows/r1.owl#r1>
        a workflow:WorkflowTemplate ;
    workflow:hasInputRole 
      <http://ontosoft.isi.edu:8080/wings-portal/export/users/
      tirth/TestingDomain/workflows/r1.owl#InputFormattedFile_irole> ;
    workflow:hasLink 
      <http://ontosoft.isi.edu:8080/wings-portal/export/users/
      tirth/TestingDomain/workflows/r1.owl#xmltotext_node_OutputTextFile_output>,

  """^^xsd:string .


###  http://www.wings-workflows.org/ontology/workflow.owl#XProduct
:XProduct rdf:type owl:Class ;
          rdfs:subClassOf :SetCreationExpression .


#################################################################
#    Annotations
#################################################################

:breakPoint rdfs:comment "The WINGS breakPoint is a WINGS workflow data property that represents a WingsWorkflowVariable always has a breakpoint."^^xsd:string ;
            rdfs:label "breakPoint"^^xsd:string .


###  Generated by the OWL API (version 5.1.0) https://github.com/owlcs/owlapi/
