@prefix : <http://www.wings-workflows.org/ontology/component.owl#> .
@prefix owl: <http://www.w3.org/2002/07/owl#> .
@prefix rdf: <http://www.w3.org/1999/02/22-rdf-syntax-ns#> .
@prefix xml: <http://www.w3.org/XML/1998/namespace> .
@prefix xsd: <http://www.w3.org/2001/XMLSchema#> .
@prefix rdfs: <http://www.w3.org/2000/01/rdf-schema#> .
@base <http://www.wings-workflows.org/ontology/component.owl> .

<http://www.wings-workflows.org/ontology/component.owl> rdf:type owl:Ontology .

#################################################################
#    Annotation properties
#################################################################

###  http://www.w3.org/2000/01/rdf-schema#comment
rdfs:comment rdf:type owl:AnnotationProperty .


###  http://www.w3.org/2004/02/skos/core#example
<http://www.w3.org/2004/02/skos/core#example> rdf:type owl:AnnotationProperty .


#################################################################
#    Object Properties
#################################################################

###  http://www.wings-workflows.org/ontology/component.owl#hasArgument
:hasArgument rdf:type owl:ObjectProperty ;
             rdfs:domain :Component ;
             rdfs:range :ComponentArgument ;
             rdfs:comment "The WINGS hasArgument is a WINGS workflow component object property that represents a connection between a WingsWorkflowComponent and the component's argument i.e. a WingsWorkflowComponent hasArgument a WingsWorkflowComponentArgument."^^xsd:string ;
             rdfs:label "hasArgument"^^xsd:string .


###  http://www.wings-workflows.org/ontology/component.owl#hasInput
:hasInput rdf:type owl:ObjectProperty ;
          rdfs:subPropertyOf :hasArgument ;
          rdfs:domain :Component ;
          rdfs:range :ComponentArgument ;
          rdfs:comment "The WINGS hasInput is a WINGS workflow component object property that represents a connection between a WingsWorkflowComponent and the component's argument i.e. a WingsWorkflowComponent hasInput a WingsWorkflowComponentArgument."^^xsd:string ;
          rdfs:label "hasInput"^^xsd:string ;
          <http://www.w3.org/2004/02/skos/core#example> """
	@prefix component_library:   <http://ontosoft.isi.edu:8080/wings-portal/export/users/tirth/TestingDomain/components/
								 library.owl#> .
	@prefix wings_component:   <http://www.wings-workflows.org/ontology/component.owl#> .

	component_library:SingleWordCount  a        component_library:SingleWordCountClass ;
	        wings_component:hasDocumentation  \"<font face=\\\"null\\\">This component counts occurrences of a single word in a 
	        								   file.</font>\" ;  								   
	       	wings_component:hasInput          component_library:SingleWordCount_number , component_library:SingleWordCount_word 
	       									  ,component_library:SingleWordCount_sampleInputFile1 ;
	        wings_component:hasOutput         component_library:SingleWordCount_outputCountFile ;
	        wings_component:isConcrete        false .
         """^^xsd:string .


###  http://www.wings-workflows.org/ontology/component.owl#hasOutput
:hasOutput rdf:type owl:ObjectProperty ;
           rdfs:subPropertyOf :hasArgument ;
           rdfs:domain :Component ;
           rdfs:range :DataArgument ;
           rdfs:comment "The WINGS hasOutput is a WINGS workflow component object property that represents a connection between a WingsWorkflowComponent and the component's data argument i.e. a WingsWorkflowComponent hasOutput a WingsWorkflowDataArgument."^^xsd:string ;
           rdfs:label "hasOutput"^^xsd:string ;
           <http://www.w3.org/2004/02/skos/core#example> """
	@prefix component_library:   <http://ontosoft.isi.edu:8080/wings-portal/export/users/tirth/TestingDomain/components/
								 library.owl#> .
	@prefix wings_component:   <http://www.wings-workflows.org/ontology/component.owl#> .

	component_library:SingleWordCount  a        component_library:SingleWordCountClass ;
	        wings_component:hasDocumentation  \"<font face=\\\"null\\\">This component counts occurrences of a single word in a 
	        								   file.</font>\" ;  								   
	       	wings_component:hasInput          component_library:SingleWordCount_number , component_library:SingleWordCount_word 
	       									  ,component_library:SingleWordCount_sampleInputFile1 ;
	        wings_component:hasOutput         component_library:SingleWordCount_outputCountFile ;
	        wings_component:isConcrete        false .
         """^^xsd:string .


#################################################################
#    Data properties
#################################################################

###  http://www.wings-workflows.org/ontology/component.owl#hasArgumentID
:hasArgumentID rdf:type owl:DatatypeProperty ,
                        owl:FunctionalProperty ;
               rdfs:domain :ComponentArgument ;
               rdfs:range xsd:string ;
               rdfs:comment "The WINGS hasArgumentID is a WINGS workflow component data property that represents a WingsWorkflowComponent having a argumentID (specified as string) for its component."^^xsd:string ;
               rdfs:label "hasArgumentID"^^xsd:string ;
               <http://www.w3.org/2004/02/skos/core#example> """
    @prefix ontology:   <http://ontosoft.isi.edu:8080/wings-portal/export/users/tirth/TestingDomain/data/ontology.owl#> .
	@prefix wings_component:   <http://www.wings-workflows.org/ontology/component.owl#> .
	@prefix component_library:   <http://ontosoft.isi.edu:8080/wings-portal/export/users/tirth/TestingDomain/components/
								 library.owl#> .	

    component_library:spacing_OutputFile1
	        a                      ontology:TextFile , wings_component:DataArgument ;
	        wings_component:hasArgumentID      \"OutputFile1\" ;
	        wings_component:hasArgumentName    \"-o1\" ;
	        wings_component:hasDimensionality  0 .
     """^^xsd:string .


###  http://www.wings-workflows.org/ontology/component.owl#hasArgumentIndex
:hasArgumentIndex rdf:type owl:DatatypeProperty ,
                           owl:FunctionalProperty ;
                  rdfs:domain :ComponentArgument ;
                  rdfs:range xsd:int ;
                  rdfs:comment "The WINGS hasArgumentIndex is a WINGS workflow component data property that represents a WingsWorkflowComponent having a argumentIndex (specified as a number(int) eg. 0,1,2,...) for its component."^^xsd:string ;
                  rdfs:label "hasArgumentIndex"^^xsd:string .


###  http://www.wings-workflows.org/ontology/component.owl#hasArgumentName
:hasArgumentName rdf:type owl:DatatypeProperty ,
                          owl:FunctionalProperty ;
                 rdfs:domain :ComponentArgument ;
                 rdfs:range xsd:string ;
                 rdfs:comment "The WINGS hasArgumentName is a WINGS workflow component data property that represents a WingsWorkflowComponent having a argumentName (specified as a string) for its component."^^xsd:string ;
                 rdfs:label "hasArgumentName"^^xsd:string ;
                 <http://www.w3.org/2004/02/skos/core#example> """
    @prefix ontology:   <http://ontosoft.isi.edu:8080/wings-portal/export/users/tirth/TestingDomain/data/ontology.owl#> .
	@prefix wings_component:   <http://www.wings-workflows.org/ontology/component.owl#> .
	@prefix component_library:   <http://ontosoft.isi.edu:8080/wings-portal/export/users/tirth/TestingDomain/components/		
								 library.owl#> .	

    component_library:spacing_OutputFile1
	        a                      ontology:TextFile , wings_component:DataArgument ;
	        wings_component:hasArgumentID      \"OutputFile1\" ;
	        wings_component:hasArgumentName    \"-o1\" ;
	        wings_component:hasDimensionality  0 .
     """^^xsd:string .


###  http://www.wings-workflows.org/ontology/component.owl#hasBindingID
:hasBindingID rdf:type owl:DatatypeProperty ,
                       owl:FunctionalProperty ;
              rdfs:domain :ComponentArgument ;
              rdfs:range xsd:string ;
              rdfs:comment "The WINGS hasBindingID is a WINGS workflow component data property that represents a WingsWorkflowComponentArgument having a ID (specified as a string) for its componentArgument."^^xsd:string ;
              rdfs:label "hasBindingID"^^xsd:string .


###  http://www.wings-workflows.org/ontology/component.owl#hasDimensionIndexProperties
:hasDimensionIndexProperties rdf:type owl:DatatypeProperty ,
                                      owl:FunctionalProperty ;
                             rdfs:domain :ComponentArgument ;
                             rdfs:range xsd:string ;
                             rdfs:comment "The WINGS hasDimensionIndexProperties is a WINGS workflow component data property that represents a WingsWorkflowComponentArgument having dimensional properties (specified as a string) for its componentArgument."^^xsd:string ;
                             rdfs:label "hasDimensionIndexProperties"^^xsd:string .


###  http://www.wings-workflows.org/ontology/component.owl#hasDimensionSizes
:hasDimensionSizes rdf:type owl:DatatypeProperty ,
                            owl:FunctionalProperty ;
                   rdfs:domain :ComponentArgument ;
                   rdfs:range xsd:string ;
                   rdfs:comment "The WINGS hasDimensionSizes is a WINGS workflow component data property that represents a WingsWorkflowComponentArgument having dimensional sizes (specified as a string) for its componentArgument."^^xsd:string ;
                   rdfs:label "hasDimensionSizes"^^xsd:string .


###  http://www.wings-workflows.org/ontology/component.owl#hasDimensionality
:hasDimensionality rdf:type owl:DatatypeProperty ,
                            owl:FunctionalProperty ;
                   rdfs:domain :ComponentArgument ;
                   rdfs:range xsd:int ;
                   rdfs:comment "The WINGS hasDimensionality is a WINGS workflow component data property that represents a WingsWorkflowComponentArgument having dimensionality (specficied as a number(int) 0,1)."^^xsd:string ;
                   rdfs:label "hasDimensionality"^^xsd:string ;
                   <http://www.w3.org/2004/02/skos/core#example> """

	@prefix wings_component:   <http://www.wings-workflows.org/ontology/component.owl#> .
	@prefix component_library:   <http://ontosoft.isi.edu:8080/wings-portal/export/users/tirth/TestingDomain/components/		
								 library.owl#> .	

    component_library:ConcrCounterNewerOne_NumberInput
	        a                      wings_component:ParameterArgument ;
	        wings_component:hasArgumentID      \"NumberInput\" ;
	        wings_component:hasArgumentName    \"-p1\" ;
	        wings_component:hasDimensionality  0 ;
	        wings_component:hasValue           0 .

    """^^xsd:string .


###  http://www.wings-workflows.org/ontology/component.owl#hasDocumentation
:hasDocumentation rdf:type owl:DatatypeProperty ;
                  rdfs:domain :Component ;
                  rdfs:range xsd:string ;
                  rdfs:comment "The WINGS hasDocumentation is a WINGS workflow component data property that represents a WingsWorkflowComponent having a documentation for its component."^^xsd:string ;
                  rdfs:label "hasDocumentation"^^xsd:string ;
                  <http://www.w3.org/2004/02/skos/core#example> """
	@prefix component_library:   <http://ontosoft.isi.edu:8080/wings-portal/export/users/tirth/TestingDomain/components/
								 library.owl#> .
	@prefix wings_component:   <http://www.wings-workflows.org/ontology/component.owl#> .

	component_library:SingleWordCount  a        component_library:SingleWordCountClass ;
	        wings_component:hasDocumentation  \"<font face=\\\"null\\\">This component counts occurrences of a single word in a 
	        								   file.</font>\" ;  								   
	       	wings_component:hasInput          component_library:SingleWordCount_number , component_library:SingleWordCount_word 
	       									  ,component_library:SingleWordCount_sampleInputFile1 ;
	        wings_component:hasOutput         component_library:SingleWordCount_outputCountFile ;
	        wings_component:isConcrete        false .
         """^^xsd:string .


###  http://www.wings-workflows.org/ontology/component.owl#hasLocation
:hasLocation rdf:type owl:DatatypeProperty ;
             rdfs:domain :Component ;
             rdfs:range xsd:string ;
             rdfs:comment "The WINGS hasLocation is a WINGS workflow component data property that represents a WingsWorkflowComponent having a location (specified as a string) for its component."^^xsd:string ;
             rdfs:label "hasLocation"^^xsd:string ;
             <http://www.w3.org/2004/02/skos/core#example> """
	@prefix component_library:   <http://ontosoft.isi.edu:8080/wings-portal/export/users/tirth/TestingDomain/components/
								 library.owl#> .
	@prefix wings_component:   <http://www.wings-workflows.org/ontology/component.owl#> .
	@prefix resource:   <http://www.wings-workflows.org/ontology/resource.owl#> .

	component_library:htmltotext  a                  component_library:htmltotextClass ;
	        wings_component:hasDocumentation       \"\" ;
	        wings_component:hasInput               component_library:htmltotext_InputFormattedFile ;
	        wings_component:hasLocation            \"/opt/wings/storage/default/users/tirth/TestingDomain/code/library/htmltotext\" ;
	        wings_component:hasOutput              component_library:htmltotext_OutputTextFile ;
	        wings_component:isConcrete             true ;
	        resource:hasHardwareDependency  [ a                      resource:HardwareDependency ;
	                                     resource:needs64bit         false ;
	                                     resource:requiresMemoryGB   \"0.0\"^^xsd:float ;
	                                     resource:requiresStorageGB  \"0.0\"^^xsd:float
	                                   ] .
         """^^xsd:string .


###  http://www.wings-workflows.org/ontology/component.owl#hasRule
:hasRule rdf:type owl:DatatypeProperty ;
         rdfs:domain :Component ;
         rdfs:range xsd:string ;
         rdfs:comment "The WINGS hasRule is a WINGS workflow component data property that represents a WingsWorkflowComponent having a rule (specified as a block of code in strings) for its component."^^xsd:string ;
         rdfs:label "hasRule"^^xsd:string ;
         <http://www.w3.org/2004/02/skos/core#example> """
	@prefix component_library:   <http://ontosoft.isi.edu:8080/wings-portal/export/users/tirth/TestingDomain/components/
								 library.owl#> .
	@prefix wings_component:   <http://www.wings-workflows.org/ontology/component.owl#> .
	@prefix resource:   <http://www.wings-workflows.org/ontology/resource.owl#> .

	component_library:breakDoc  a                    component_library:breakDocClass ;
	        wings_component:hasInput               component_library:breakDoc_nToBreakInto , component_library:breakDoc_InputFile1 ;
	        wings_component:hasLocation            \"/opt/wings/storage/default/users/tirth/TestingDomain/code/library/breakDoc\" ;
	        wings_component:hasOutput              component_library:breakDoc_OutputFiles ;
	        wings_component:hasRule                \"[ SetOutputCollectionSize: (?c rdf:type acdom:breakDocClass) (?c ac:hasInput ?idv) (?idv ac:hasArgumentID 'InputFile1') (?c ac:hasInput ?ipv) (?ipv ac:hasArgumentID 'nToBreakInto') (?c ac:hasOutput ?odv) (?odv ac:hasArgumentID 'OutputFiles') (?ipv ac:hasValue ?num) -> (?odv ac:hasDimensionSizes ?num) print(Breaking ?idv into ?num files) ]\" ;
	        wings_component:isConcrete             true ;
	        resource:hasHardwareDependency  [ a                      resource:HardwareDependency ;
	                                     resource:needs64bit         false ;
	                                     resource:requiresMemoryGB   \"0.0\"^^xsd:float ;
	                                     resource:requiresStorageGB  \"0.0\"^^xsd:float
	                                   ] .
	         """^^xsd:string .


###  http://www.wings-workflows.org/ontology/component.owl#hasValue
:hasValue rdf:type owl:DatatypeProperty ,
                   owl:FunctionalProperty ;
          rdfs:domain :ParameterArgument ;
          rdfs:comment "The WINGS hasValue is a WINGS workflow component data property that represents a WingsWorkflowComponentParameterArgument having a value for the parameter."^^xsd:string ;
          rdfs:label "hasValue"^^xsd:string ;
          <http://www.w3.org/2004/02/skos/core#example> """
   	@prefix wings_component:   <http://www.wings-workflows.org/ontology/component.owl#> .
	@prefix component_library:   <http://ontosoft.isi.edu:8080/wings-portal/export/users/tirth/TestingDomain/components/		
								 library.owl#> .	

    component_library:ConcrCounterNewerOne_NumberInput
	        a                      wings_component:ParameterArgument ;
	        wings_component:hasArgumentID      \"NumberInput\" ;
	        wings_component:hasArgumentName    \"-p1\" ;
	        wings_component:hasDimensionality  0 ;
	        wings_component:hasValue           0 .

    """^^xsd:string .


###  http://www.wings-workflows.org/ontology/component.owl#isConcrete
:isConcrete rdf:type owl:DatatypeProperty ,
                     owl:FunctionalProperty ;
            rdfs:domain :Component ;
            rdfs:range xsd:boolean ;
            rdfs:comment "The WINGS isConcrete is a WINGS workflow component data property that represents a WingsWorkflowComponent is abstract or not. If it is abstract then the value is false, else its true. (range is boolean) "^^xsd:string ;
            rdfs:label "isConcrete"^^xsd:string ;
            <http://www.w3.org/2004/02/skos/core#example> """
   	@prefix wings_component:   <http://www.wings-workflows.org/ontology/component.owl#> .
	@prefix component_library:   <http://ontosoft.isi.edu:8080/wings-portal/export/users/tirth/TestingDomain/components/		
								 library.owl#> .	

	component_library:TRIALCONCR  a       component_library:TRIALCONCRClass ;
	        wings_component:hasInput    component_library:TRIALCONCR_InputWord , component_library:TRIALCONCR_InputFile ;
	        wings_component:hasOutput   component_library:TRIALCONCR_OutputFile ;
	        wings_component:isConcrete  false .
    """^^xsd:string .


###  http://www.wings-workflows.org/ontology/component.owl#isInvalid
:isInvalid rdf:type owl:DatatypeProperty ,
                    owl:FunctionalProperty ;
           rdfs:domain :Component ;
           rdfs:range xsd:boolean ;
           rdfs:comment "The WINGS isInvalid is a WINGS workflow component data property that represents a WingsWorkflowComponent is either valid or not."^^xsd:string ;
           rdfs:label "isInvalid"^^xsd:string .


#################################################################
#    Classes
#################################################################

###  http://www.wings-workflows.org/ontology/component.owl#Component
:Component rdf:type owl:Class ;
           rdfs:comment "The WINGS Component is a WINGS component class that represents a component of WINGS Workflow template specification."^^xsd:string ;
           rdfs:label "Component"^^xsd:string ;
           <http://www.w3.org/2004/02/skos/core#example> """
   	@prefix wings_component:   <http://www.wings-workflows.org/ontology/component.owl#> .
	@prefix component_library:   <http://ontosoft.isi.edu:8080/wings-portal/export/users/tirth/TestingDomain/components/		
								 library.owl#> .	

    component_library:splitClass
	      	a        owl:Class ;
	        rdfs:subClassOf  
	        	wings_component:Component .
    """^^xsd:string .


###  http://www.wings-workflows.org/ontology/component.owl#ComponentArgument
:ComponentArgument rdf:type owl:Class ;
                   rdfs:comment "The WINGS ComponentArgument is a WINGS component class that represents a componentArgument in the  WINGS Workflow template specification."^^xsd:string ;
                   rdfs:label "ComponentArgument"^^xsd:string .


###  http://www.wings-workflows.org/ontology/component.owl#DataArgument
:DataArgument rdf:type owl:Class ;
              rdfs:subClassOf :ComponentArgument ;
              rdfs:comment "The WINGS DataArgument is a WINGS component class that represents a data based argument and it has the Component argument as a subclass."^^xsd:string ;
              rdfs:label "DataArgument"^^xsd:string ;
              <http://www.w3.org/2004/02/skos/core#example> """
	@prefix data_ontology:   <http://ontosoft.isi.edu:8080/wings-portal/export/users/tirth/TestingDomain/data/ontology.owl#> .
    @prefix wings_component:   <http://www.wings-workflows.org/ontology/component.owl#> .
	@prefix component_library:   <http://ontosoft.isi.edu:8080/wings-portal/export/users/tirth/TestingDomain/components/		
								 library.owl#> .	

	component_library:Convert_OutputFile
	        a                      data_ontology:TextFile , wings_component:DataArgument ;
	        wings_component:hasArgumentID      \"OutputFile\" ;
	        wings_component:hasArgumentName    \"-o1\" ;
	        wings_component:hasDimensionality  0 .

    """^^xsd:string .


###  http://www.wings-workflows.org/ontology/component.owl#ParameterArgument
:ParameterArgument rdf:type owl:Class ;
                   rdfs:subClassOf :ComponentArgument ;
                   rdfs:comment "The WINGS ParameterArgument is a WINGS component class that represents a parameter based argument and it has the Component argument as a subclass."^^xsd:string ;
                   rdfs:label "ParameterArgument"^^xsd:string ;
                   <http://www.w3.org/2004/02/skos/core#example> """
	@prefix wings_component:   <http://www.wings-workflows.org/ontology/component.owl#> .
	@prefix component_library: <http://ontosoft.isi.edu:8080/wings-portal/export/users/tirth/TestingDomain/components/		
							   library.owl#> .	

	component_library:count3_LetterInput
			a                      wings_component:ParameterArgument ;
			wings_component:hasArgumentID      \"LetterInput\" ;
			wings_component:hasArgumentName    \"-p3\" ;
			wings_component:hasDimensionality  0 ;
			wings_component:hasValue           \"\" .
    """^^xsd:string .


###  Generated by the OWL API (version 5.1.0) https://github.com/owlcs/owlapi/
