@prefix : <http://www.wings-workflows.org/ontology/component.owl#> .
@prefix owl: <http://www.w3.org/2002/07/owl#> .
@prefix rdf: <http://www.w3.org/1999/02/22-rdf-syntax-ns#> .
@prefix xml: <http://www.w3.org/XML/1998/namespace> .
@prefix xsd: <http://www.w3.org/2001/XMLSchema#> .
@prefix rdfs: <http://www.w3.org/2000/01/rdf-schema#> .
@base <http://www.wings-workflows.org/ontology/component.owl> .

<http://www.wings-workflows.org/ontology/component.owl> rdf:type owl:Ontology .

#################################################################
#    Annotation properties
#################################################################

###  http://www.w3.org/2000/01/rdf-schema#comment
rdfs:comment rdf:type owl:AnnotationProperty .


###  http://www.w3.org/2004/02/skos/core#example
<http://www.w3.org/2004/02/skos/core#example> rdf:type owl:AnnotationProperty .


#################################################################
#    Object Properties
#################################################################

###  http://www.wings-workflows.org/ontology/component.owl#hasArgument
:hasArgument rdf:type owl:ObjectProperty ;
             rdfs:domain :Component ;
             rdfs:range :ComponentArgument ;
             rdfs:comment "The WINGS hasArgument is a WINGS workflow component object property that represents a connection between a WingsWorkflowComponent and the component's argument i.e. a WingsWorkflowComponent hasArgument a WingsWorkflowComponentArgument."^^xsd:string ;
             rdfs:label "hasArgument"^^xsd:string .


###  http://www.wings-workflows.org/ontology/component.owl#hasInput
:hasInput rdf:type owl:ObjectProperty ;
          rdfs:subPropertyOf :hasArgument ;
          rdfs:domain :Component ;
          rdfs:range :ComponentArgument ;
          rdfs:comment "The WINGS hasInput is a WINGS workflow component object property that represents a connection between a WingsWorkflowComponent and the component's argument i.e. a WingsWorkflowComponent hasInput a WingsWorkflowComponentArgument."^^xsd:string ;
          rdfs:label "hasInput"^^xsd:string .


###  http://www.wings-workflows.org/ontology/component.owl#hasOutput
:hasOutput rdf:type owl:ObjectProperty ;
           rdfs:subPropertyOf :hasArgument ;
           rdfs:domain :Component ;
           rdfs:range :DataArgument ;
           rdfs:comment "The WINGS hasOutput is a WINGS workflow component object property that represents a connection between a WingsWorkflowComponent and the component's data argument i.e. a WingsWorkflowComponent hasOutput a WingsWorkflowDataArgument."^^xsd:string ;
           rdfs:label "hasOutput"^^xsd:string .


#################################################################
#    Data properties
#################################################################

###  http://www.wings-workflows.org/ontology/component.owl#hasArgumentID
:hasArgumentID rdf:type owl:DatatypeProperty ,
                        owl:FunctionalProperty ;
               rdfs:domain :ComponentArgument ;
               rdfs:range xsd:string ;
               rdfs:comment "The WINGS hasArgumentID is a WINGS workflow component data property that represents a WingsWorkflowComponent having a argumentID (specified as string) for its component."^^xsd:string ;
               rdfs:label "hasArgumentID"^^xsd:string .


###  http://www.wings-workflows.org/ontology/component.owl#hasArgumentIndex
:hasArgumentIndex rdf:type owl:DatatypeProperty ,
                           owl:FunctionalProperty ;
                  rdfs:domain :ComponentArgument ;
                  rdfs:range xsd:int ;
                  rdfs:comment "The WINGS hasArgumentIndex is a WINGS workflow component data property that represents a WingsWorkflowComponent having a argumentIndex (specified as a number(int) eg. 0,1,2,...) for its component."^^xsd:string ;
                  rdfs:label "hasArgumentIndex"^^xsd:string .


###  http://www.wings-workflows.org/ontology/component.owl#hasArgumentName
:hasArgumentName rdf:type owl:DatatypeProperty ,
                          owl:FunctionalProperty ;
                 rdfs:domain :ComponentArgument ;
                 rdfs:range xsd:string ;
                 rdfs:comment "The WINGS hasArgumentName is a WINGS workflow component data property that represents a WingsWorkflowComponent having a argumentName (specified as a string) for its component."^^xsd:string ;
                 rdfs:label "hasArgumentName"^^xsd:string .


###  http://www.wings-workflows.org/ontology/component.owl#hasBindingID
:hasBindingID rdf:type owl:DatatypeProperty ,
                       owl:FunctionalProperty ;
              rdfs:domain :ComponentArgument ;
              rdfs:range xsd:string ;
              rdfs:comment "The WINGS hasBindingID is a WINGS workflow component data property that represents a WingsWorkflowComponentArgument having a bindingID (specified as a string) for its componentArgument."^^xsd:string ;
              rdfs:label "hasBindingID"^^xsd:string .


###  http://www.wings-workflows.org/ontology/component.owl#hasDimensionIndexProperties
:hasDimensionIndexProperties rdf:type owl:DatatypeProperty ,
                                      owl:FunctionalProperty ;
                             rdfs:domain :ComponentArgument ;
                             rdfs:range xsd:string ;
                             rdfs:comment "The WINGS hasDimensionIndexProperties is a WINGS workflow component data property that represents a WingsWorkflowComponentArgument having dimensional index properties (specified as a string) for its componentArgument."^^xsd:string ;
                             rdfs:label "hasDimensionIndexProperties"^^xsd:string .


###  http://www.wings-workflows.org/ontology/component.owl#hasDimensionSizes
:hasDimensionSizes rdf:type owl:DatatypeProperty ,
                            owl:FunctionalProperty ;
                   rdfs:domain :ComponentArgument ;
                   rdfs:range xsd:string ;
                   rdfs:comment "The WINGS hasDimensionSizes is a WINGS workflow component data property that represents a WingsWorkflowComponentArgument having dimemsional sizes (specified as a string) for its componentArgument."^^xsd:string ;
                   rdfs:label "hasDimensionSizes"^^xsd:string .


###  http://www.wings-workflows.org/ontology/component.owl#hasDimensionality
:hasDimensionality rdf:type owl:DatatypeProperty ,
                            owl:FunctionalProperty ;
                   rdfs:domain :ComponentArgument ;
                   rdfs:range xsd:int ;
                   rdfs:comment "The WINGS hasDimensionality is a WINGS workflow component data property that represents a WingsWorkflowComponentArgument having dimensionality (specficied as a number(int) 0,1)."^^xsd:string ;
                   rdfs:label "hasDimensionality"^^xsd:string ;
                   <http://www.w3.org/2004/02/skos/core#example> """
	        <https://w3id.org/wings/TestingDomain#INPUTFILE>
	        a  <https://w3id.org/wings/TestingDomain/Data/TextFile> ,
	           <https://w3id.org/wings/TestingDomain/Data/DataArgument> ,
	           <https://w3id.org/wings/TestingDomain#TextFile> ,
	           <https://w3id.org/wings/TestingDomain#DataArgument> ;
	        
            <http://www.wings-workflows.org/ontology/component.owl#hasArgumentID>
	                \"InputFile\" ;
	        <http://www.wings-workflows.org/ontology/component.owl#hasArgumentName>
	                \"-i1\" ;
	        <http://www.wings-workflows.org/ontology/component.owl#hasDimensionality>
	                \"0\"^^xsd:int .
    """^^xsd:string .


###  http://www.wings-workflows.org/ontology/component.owl#hasDocumentation
:hasDocumentation rdf:type owl:DatatypeProperty ;
                  rdfs:domain :Component ;
                  rdfs:range xsd:string ;
                  rdfs:comment "The WINGS hasDocumentation is a WINGS workflow component data property that represents a WingsWorkflowComponent having a documentation for its component."^^xsd:string ;
                  rdfs:label "hasDocumentation"^^xsd:string .


###  http://www.wings-workflows.org/ontology/component.owl#hasLocation
:hasLocation rdf:type owl:DatatypeProperty ;
             rdfs:domain :Component ;
             rdfs:range xsd:string ;
             rdfs:comment "The WINGS hasLocation is a WINGS workflow component data property that represents a WingsWorkflowComponent having a location (specified as a string) for its component."^^xsd:string ;
             rdfs:label "hasLocation"^^xsd:string .


###  http://www.wings-workflows.org/ontology/component.owl#hasRule
:hasRule rdf:type owl:DatatypeProperty ;
         rdfs:domain :Component ;
         rdfs:range xsd:string ;
         rdfs:comment "The WINGS hasRule is a WINGS workflow component data property that represents a WingsWorkflowComponent having a rule (specified as a block of code in strings) for its component."^^xsd:string ;
         rdfs:label "hasRule"^^xsd:string .


###  http://www.wings-workflows.org/ontology/component.owl#hasValue
:hasValue rdf:type owl:DatatypeProperty ,
                   owl:FunctionalProperty ;
          rdfs:domain :ParameterArgument ;
          rdfs:comment "The WINGS hasValue is a WINGS workflow component data property that represents a WingsWorkflowComponentParameterArgument having a value for the parameter."^^xsd:string ;
          rdfs:label "hasValue"^^xsd:string .


###  http://www.wings-workflows.org/ontology/component.owl#isConcrete
:isConcrete rdf:type owl:DatatypeProperty ,
                     owl:FunctionalProperty ;
            rdfs:domain :Component ;
            rdfs:range xsd:boolean ;
            rdfs:comment "The WINGS isConcrete is a WINGS workflow component data property that represents a WingsWorkflowComponent is abstract or not. If it is abstract then the value is false, else its true. (range is boolean) "^^xsd:string ;
            rdfs:label "isConcrete"^^xsd:string ;
            <http://www.w3.org/2004/02/skos/core#example> """
        <https://w3id.org/wings/TestingDomain#SORT_V1>
        a           <https://w3id.org/wings/TestingDomain#SORT_CLASSV1> ;
        			rdfs:label  \"SORT\" ;
        <http://www.w3.org/ns/prov#wasAttributedTo>
                \"tirth\" ;
        <http://www.wings-workflows.org/ontology/component.owl#hasDocumentation>
                \"\" ;
                
        <http://www.wings-workflows.org/ontology/component.owl#hasInput>
            <https://w3id.org/wings/TestingDomain#INPUTFILE> ,
            <https://w3id.org/wings/TestingDomain#INPUTWORD> ,
            <https://w3id.org/wings/TestingDomain#SECOND-INPUTFILE> ;

        <http://www.wings-workflows.org/ontology/component.owl#hasOutput>
            <https://w3id.org/wings/TestingDomain#OUTPUTFILE> ;
        <http://www.wings-workflows.org/ontology/component.owl#isConcrete>
                false .
    """^^xsd:string .


###  http://www.wings-workflows.org/ontology/component.owl#isInvalid
:isInvalid rdf:type owl:DatatypeProperty ,
                    owl:FunctionalProperty ;
           rdfs:domain :Component ;
           rdfs:range xsd:boolean ;
           rdfs:comment "The WINGS isInvalid is a WINGS workflow component data property that represents a WingsWorkflowComponent is either valid or not."^^xsd:string ;
           rdfs:label "isInvalid"^^xsd:string .


#################################################################
#    Classes
#################################################################

###  http://www.wings-workflows.org/ontology/component.owl#Component
:Component rdf:type owl:Class ;
           rdfs:comment "The WINGS Component is a WINGS component class that represents a component of WINGS Workflow template specification."^^xsd:string ;
           rdfs:label "Component"^^xsd:string .


###  http://www.wings-workflows.org/ontology/component.owl#ComponentArgument
:ComponentArgument rdf:type owl:Class ;
                   rdfs:comment "The WINGS ComponentArgument is a WINGS component class that represents a componentArgument in the  WINGS Workflow template specification."^^xsd:string ;
                   rdfs:label "ComponentArgument"^^xsd:string .


###  http://www.wings-workflows.org/ontology/component.owl#DataArgument
:DataArgument rdf:type owl:Class ;
              rdfs:subClassOf :ComponentArgument ;
              rdfs:comment "The WINGS DataArgument is a WINGS component class that represents a data based argument and it has the Component argument as a subclass."^^xsd:string ;
              rdfs:label "DataArgument"^^xsd:string .


###  http://www.wings-workflows.org/ontology/component.owl#ParameterArgument
:ParameterArgument rdf:type owl:Class ;
                   rdfs:subClassOf :ComponentArgument ;
                   rdfs:comment "The WINGS ParameterArgument is a WINGS component class that represents a parameter based argument and it has the Component argument as a subclass."^^xsd:string ;
                   rdfs:label "ParameterArgument"^^xsd:string .


###  Generated by the OWL API (version 5.1.0) https://github.com/owlcs/owlapi/
